WIP

src/tlogic/MonotoneRA.v
@@ -1,5 +1,5 @@
 From sflib Require Import sflib.
-From Fairness Require Import PCM IProp IPM.
+From Fairness Require Import PCM IProp IPM IPropAux.
 Require Import Coq.Classes.RelationClasses.
 Require Import Coq.Logic.PropExtensionality.
 From Fairness Require Import Axioms.
@@ -333,49 +333,6 @@ Qed.
 
 
 
-Lemma embed_core_commute `{@GRA.inG M Σ}
-      (r: M)
-  :
-  GRA.embed (URA.core r) = URA.core (GRA.embed r).
-Proof.
-  Local Transparent GRA.to_URA URA.unit.
-  dependent destruction H. subst.
-  extensionality n. ss. unfold URA.core at 2. ss.
-  unfold GRA.embed. destruct (PeanoNat.Nat.eq_dec GRA.inG_id n) eqn:EQ; ss.
-  { subst. ss. }
-  { des_ifs. ss. transitivity (add (core unit) unit); auto. }
-Qed.
-
-Lemma own_persistent `{@GRA.inG M Σ}
-      (r: M)
-  :
-  (OwnM r) -∗ (□ OwnM (URA.core r)).
-Proof.
-  rr. autorewrite with iprop. i.
-  rr. autorewrite with iprop. split.
-  { rr. autorewrite with iprop. auto. }
-  { rr. autorewrite with iprop.
-    rr in H0. autorewrite with iprop in H0.
-    rr. autorewrite with iprop.
-    eapply URA.extends_core in H0.
-    rewrite embed_core_commute. auto.
-  }
-Qed.
-
-Lemma OwnM_unit `{@GRA.inG M Σ}
-  :
-  ⊢ OwnM (@URA.unit M).
-Proof.
-  rr. autorewrite with iprop. i.
-  rr. autorewrite with iprop.
-  exists r.
-  Local Transparent GRA.to_URA URA.unit.
-  replace (GRA.embed ε) with (@URA.unit Σ).
-  { rewrite URA.unit_idl. auto. }
-  unfold GRA.embed. extensionality n. des_ifs. ss.
-  destruct H. ss. destruct inG_prf. ss.
-Qed.
-
 Section Monotone.
   Definition monoRA: URA.t := @FiniteMap.t (Auth.t (Collection.t gmon)).
   Context `{@GRA.inG monoRA Σ}.
@@ -544,120 +501,120 @@ Section Monotone.
 End Monotone.
 
 
-Section Monotone.
-  Variable W: Type.
-  Variable le: W -> W -> Prop.
-  Hypothesis le_PreOrder: PreOrder le.
+(* Section Monotone. *)
+(*   Variable W: Type. *)
+(*   Variable le: W -> W -> Prop. *)
+(*   Hypothesis le_PreOrder: PreOrder le. *)
 
-  Let leR (w: W): Collection.t W := le w.
+(*   Let leR (w: W): Collection.t W := le w. *)
 
-  Definition monoRA2: URA.t := Auth.t (Collection.t W).
+(*   Definition monoRA2: URA.t := Auth.t (Collection.t W). *)
 
-  Context `{@GRA.inG monoRA2 Σ}.
+(*   Context `{@GRA.inG monoRA2 Σ}. *)
 
-  Definition monoBlack2 (w: W): iProp :=
-    OwnM (Auth.black (leR w) ⋅ Auth.white (leR w)).
+(*   Definition monoBlack2 (w: W): iProp := *)
+(*     OwnM (Auth.black (leR w) ⋅ Auth.white (leR w)). *)
 
-  Definition monoWhiteExact2 (w: W): iProp :=
-    OwnM (Auth.white (leR w)).
+(*   Definition monoWhiteExact2 (w: W): iProp := *)
+(*     OwnM (Auth.white (leR w)). *)
 
-  Definition monoWhite2 (w0: W): iProp :=
-    ∃ w1, monoWhiteExact2 w1 ∧ ⌜le w0 w1⌝.
+(*   Definition monoWhite2 (w0: W): iProp := *)
+(*     ∃ w1, monoWhiteExact2 w1 ∧ ⌜le w0 w1⌝. *)
 
-  Lemma white_exact_persistent2 w
-    :
-    (monoWhiteExact2 w) -∗ (□ monoWhiteExact2 w).
-  Proof.
-    unfold monoBlack2, monoWhiteExact2.
-    iIntros "H". iPoseProof (own_persistent with "H") as "H". ss.
-  Qed.
+(*   Lemma white_exact_persistent2 w *)
+(*     : *)
+(*     (monoWhiteExact2 w) -∗ (□ monoWhiteExact2 w). *)
+(*   Proof. *)
+(*     unfold monoBlack2, monoWhiteExact2. *)
+(*     iIntros "H". iPoseProof (own_persistent with "H") as "H". ss. *)
+(*   Qed. *)
 
-  Global Program Instance Persistent_white_exact2 w: Persistent (monoWhiteExact2 w).
-  Next Obligation.
-  Proof.
-    i. iIntros "WHITE". iPoseProof (white_exact_persistent2 with "WHITE") as "WHITE". auto.
-  Qed.
+(*   Global Program Instance Persistent_white_exact2 w: Persistent (monoWhiteExact2 w). *)
+(*   Next Obligation. *)
+(*   Proof. *)
+(*     i. iIntros "WHITE". iPoseProof (white_exact_persistent2 with "WHITE") as "WHITE". auto. *)
+(*   Qed. *)
 
-  Lemma white_persistent2 w
-    :
-    (monoWhite2 w) -∗ (□ monoWhite2 w).
-  Proof.
-    unfold monoWhite2. iIntros "H".
-    iDestruct "H" as (w1) "[H %]".
-    iPoseProof (white_exact_persistent2 with "H") as "# H0".
-    iClear "∗". iModIntro.
-    iExists _. iSplit; eauto.
-  Qed.
+(*   Lemma white_persistent2 w *)
+(*     : *)
+(*     (monoWhite2 w) -∗ (□ monoWhite2 w). *)
+(*   Proof. *)
+(*     unfold monoWhite2. iIntros "H". *)
+(*     iDestruct "H" as (w1) "[H %]". *)
+(*     iPoseProof (white_exact_persistent2 with "H") as "# H0". *)
+(*     iClear "∗". iModIntro. *)
+(*     iExists _. iSplit; eauto. *)
+(*   Qed. *)
 
-  Global Program Instance Persistent_white2 w: Persistent (monoWhite2 w).
+(*   Global Program Instance Persistent_white2 w: Persistent (monoWhite2 w). *)
 
-  Lemma black_white_exact2 w
-    :
-    (monoBlack2 w) -∗ (monoWhiteExact2 w).
-  Proof.
-    unfold monoBlack2, monoWhiteExact2.
-    iIntros "[_ H]". ss.
-  Qed.
+(*   Lemma black_white_exact2 w *)
+(*     : *)
+(*     (monoBlack2 w) -∗ (monoWhiteExact2 w). *)
+(*   Proof. *)
+(*     unfold monoBlack2, monoWhiteExact2. *)
+(*     iIntros "[_ H]". ss. *)
+(*   Qed. *)
 
-  Lemma black_white2 w
-    :
-    (monoBlack2 w) -∗ (monoWhite2 w).
-  Proof.
-    unfold monoWhite2. iIntros "H".
-    iPoseProof (black_white_exact2 with "H") as "H".
-    iExists _. iSplit; eauto.
-  Qed.
+(*   Lemma black_white2 w *)
+(*     : *)
+(*     (monoBlack2 w) -∗ (monoWhite2 w). *)
+(*   Proof. *)
+(*     unfold monoWhite2. iIntros "H". *)
+(*     iPoseProof (black_white_exact2 with "H") as "H". *)
+(*     iExists _. iSplit; eauto. *)
+(*   Qed. *)
 
-  Lemma white_mon2 w0 w1
-    :
-    (monoWhite2 w1) -∗ ⌜le w0 w1⌝ -∗ (monoWhite2 w0).
-  Proof.
-    unfold monoWhite2. iIntros "H %".
-    iDestruct "H" as (w) "[H %]".
-    iExists _. iSplit; eauto. iPureIntro. etrans; eauto.
-  Qed.
+(*   Lemma white_mon2 w0 w1 *)
+(*     : *)
+(*     (monoWhite2 w1) -∗ ⌜le w0 w1⌝ -∗ (monoWhite2 w0). *)
+(*   Proof. *)
+(*     unfold monoWhite2. iIntros "H %". *)
+(*     iDestruct "H" as (w) "[H %]". *)
+(*     iExists _. iSplit; eauto. iPureIntro. etrans; eauto. *)
+(*   Qed. *)
 
-  Lemma black_updatable2 w0 w1
-        (LE: le w0 w1)
-    :
-    (monoBlack2 w0) -∗ (#=> monoBlack2 w1).
-  Proof.
-    iIntros "H". iApply (OwnM_Upd with "H").
-    eapply Auth.auth_update.
-    rr. i. des. splits; auto.
-    { rr. unseal "ra". ss. }
-    { unfold URA.add in *. unseal "ra". ss.
-      unfold Collection.add in *.
-      extensionality w. eapply equal_f with (x:=w) in FRAME.
-      eapply prop_ext_rev in FRAME. des.
-      eapply propositional_extensionality. split; i; des; ss.
-      split; eauto. eapply FRAME. etrans; eauto.
-    }
-  Qed.
+(*   Lemma black_updatable2 w0 w1 *)
+(*         (LE: le w0 w1) *)
+(*     : *)
+(*     (monoBlack2 w0) -∗ (#=> monoBlack2 w1). *)
+(*   Proof. *)
+(*     iIntros "H". iApply (OwnM_Upd with "H"). *)
+(*     eapply Auth.auth_update. *)
+(*     rr. i. des. splits; auto. *)
+(*     { rr. unseal "ra". ss. } *)
+(*     { unfold URA.add in *. unseal "ra". ss. *)
+(*       unfold Collection.add in *. *)
+(*       extensionality w. eapply equal_f with (x:=w) in FRAME. *)
+(*       eapply prop_ext_rev in FRAME. des. *)
+(*       eapply propositional_extensionality. split; i; des; ss. *)
+(*       split; eauto. eapply FRAME. etrans; eauto. *)
+(*     } *)
+(*   Qed. *)
 
-  Lemma black_white_exact_compare2 w0 w1
-    :
-    (monoWhiteExact2 w0) -∗ (monoBlack2 w1) -∗ ⌜le w0 w1⌝.
-  Proof.
-    iIntros "H0 [H1 H2]".
-    iCombine "H1 H0" as "H". iOwnWf "H".
-    iPureIntro. eapply Auth.auth_included in H0.
-    rr in H0. des. unfold URA.add in H0. unseal "ra".
-    ss. unfold Collection.add in H0.
-    eapply equal_f in H0. eapply prop_ext_rev in H0. des.
-    eapply H1. reflexivity.
-  Qed.
+(*   Lemma black_white_exact_compare2 w0 w1 *)
+(*     : *)
+(*     (monoWhiteExact2 w0) -∗ (monoBlack2 w1) -∗ ⌜le w0 w1⌝. *)
+(*   Proof. *)
+(*     iIntros "H0 [H1 H2]". *)
+(*     iCombine "H1 H0" as "H". iOwnWf "H". *)
+(*     iPureIntro. eapply Auth.auth_included in H0. *)
+(*     rr in H0. des. unfold URA.add in H0. unseal "ra". *)
+(*     ss. unfold Collection.add in H0. *)
+(*     eapply equal_f in H0. eapply prop_ext_rev in H0. des. *)
+(*     eapply H1. reflexivity. *)
+(*   Qed. *)
 
-  Lemma black_white_compare2 w0 w1
-    :
-    (monoWhite2 w0) -∗ (monoBlack2 w1) -∗ ⌜le w0 w1⌝.
-  Proof.
-    unfold monoWhite2.
-    iIntros "H0 H1". iDestruct "H0" as (w) "[H0 %]".
-    iPoseProof (black_white_exact_compare2 with "H0 H1") as "%".
-    iPureIntro. etrans; eauto.
-  Qed.
-End Monotone.
+(*   Lemma black_white_compare2 w0 w1 *)
+(*     : *)
+(*     (monoWhite2 w0) -∗ (monoBlack2 w1) -∗ ⌜le w0 w1⌝. *)
+(*   Proof. *)
+(*     unfold monoWhite2. *)
+(*     iIntros "H0 H1". iDestruct "H0" as (w) "[H0 %]". *)
+(*     iPoseProof (black_white_exact_compare2 with "H0 H1") as "%". *)
+(*     iPureIntro. etrans; eauto. *)
+(*   Qed. *)
+(* End Monotone. *)
 
 
 Section MAP.
@@ -715,778 +672,778 @@ From iris.bi Require Import derived_laws. Import bi.
 Require Export Coq.Sorting.Mergesort. Import NatSort.
 
 
-Create HintDb mset.
-Section MUPD.
-  Definition mset := list nat.
-  Definition mset_disjoint (s0 s1: mset): Prop :=
-    forall n (IN0: List.In n s0) (IN1: List.In n s1), False.
-
-  Fixpoint mset_disjoint_b (s0 s1: mset): bool :=
-    match s0 with
-    | [] => true
-    | hd::tl =>
-        match find (Nat.eqb hd) s1 with
-        | Some _ => false
-        | None => mset_disjoint_b tl s1
-        end
-    end.
-
-  Lemma mset_disjoint_b_reflect s0 s1
-    :
-    mset_disjoint s0 s1 <-> mset_disjoint_b s0 s1 = true.
-  Proof.
-    induction s0; ss.
-    { split; i; auto. ii. inv IN0. }
-    des_ifs.
-    { split; i.
-      { eapply find_some in Heq. des.
-        rewrite Nat.eqb_eq in Heq0. subst.
-        exfalso. eapply H; eauto. econs; ss.
-      }
-      { ii. inv IN0; eauto. }
-    }
-    { rewrite <- IHs0. split; i.
-      { ii. eapply H; eauto. econs 2; ss. }
-      { ii. inv IN0.
-        { eapply find_none in Heq; eauto. rewrite Nat.eqb_refl in Heq. ss. }
-        { eapply H; eauto. }
-      }
-    }
-  Qed.
-
-  Definition list_sub A (s0 s1: list A): Prop :=
-    exists s, Permutation (s ++ s0) s1.
-
-  Global Program Instance list_sub_PreOrder A: PreOrder (@list_sub A).
-  Next Obligation.
-  Proof.
-    ii. exists []. ss.
-  Qed.
-  Next Obligation.
-  Proof.
-    ii. unfold list_sub in *. des.
-    rewrite <- H in H0. exists (s ++ s0).
-    rewrite <- app_assoc. auto.
-  Qed.
-
-  Global Instance permutation_list_sub_proper A:
-    Proper (Permutation ==> Permutation ==> iff) (@list_sub A).
-  Proof.
-    ii. unfold list_sub. split.
-    { i. des. exists s. rewrite <- H. rewrite H1. auto. }
-    { i. des. exists s. rewrite H0. rewrite H. auto. }
-  Qed.
-
-  Definition mset_sub (s0 s1: mset): Prop := list_sub s0 s1.
-
-  Global Program Instance mset_sub_PreOrder: PreOrder mset_sub.
-
-  Global Instance permutation_mset_sub_proper:
-    Proper (Permutation ==> Permutation ==> iff) mset_sub.
-  Proof.
-    unfold mset_sub. typeclasses eauto.
-  Qed.
-
-  Global Instance permutation_mset_disjoint_proper:
-    Proper (Permutation ==> Permutation ==> iff) mset_disjoint.
-  Proof.
-    ii. split.
-    { ii. eapply H1.
-      { symmetry in H. eapply Permutation_in; eauto. }
-      { symmetry in H0. eapply Permutation_in; eauto. }
-    }
-    { ii. eapply H1.
-      { eapply Permutation_in; eauto. }
-      { eapply Permutation_in; eauto. }
-    }
-  Qed.
-
-  Definition mset_minus (s0 s1: mset): mset :=
-    match list_remove_list s1 s0 with
-    | Some s => s
-    | None => []
-    end.
-
-  Definition mset_sub_b (s0 s1: mset): bool :=
-    match list_remove_list s0 s1 with
-    | Some _ => true
-    | None => false
-    end.
-
-  Lemma list_remove_none A `{EqDecision A} (a: A) (l: list A)
-        (NONE: list_remove a l = None)
-    :
-    ~ List.In a l.
-  Proof.
-    revert NONE. induction l; ss.
-    des_ifs. i. unfold fmap, option_fmap, option_map in NONE.
-    des_ifs. ii. des; clarify. eapply IHl; auto.
-  Qed.
-
-  Lemma mset_sub_b_reflect s0 s1
-    :
-    mset_sub s0 s1 <-> mset_sub_b s0 s1 = true.
-  Proof.
-    revert s1. induction s0; ss; i.
-    { split; i; auto. exists s1. rewrite app_nil_r. auto. }
-    { unfold mset_sub_b in *. ss.
-      destruct (list_remove a s1) eqn:EQ; ss.
-      { eapply list_remove_Some in EQ.
-        rewrite <- IHs0. unfold mset_sub, list_sub. split.
-        { i. des. rewrite EQ in H.
-          rewrite <- Permutation_middle in H.
-          apply Permutation_cons_inv in H.
-          exists s. auto.
-        }
-        { i. des. rewrite <- H in EQ.
-          eexists s. rewrite EQ. rewrite <- Permutation_middle. auto.
-        }
-      }
-      { eapply list_remove_none in EQ. split; i; ss.
-        exfalso. unfold mset_sub, list_sub in H. des.
-        rewrite <- Permutation_middle in H.
-        eapply EQ. eapply Permutation_in; eauto.
-        econs; ss.
-      }
-    }
-  Qed.
-
-  Context `{Σ: GRA.t}.
-  Variable I: nat -> iProp.
-  Variable IA: iProp.
-  Definition mset_all (l: mset) := fold_right (fun n P => I n ** P) True%I l.
-
-  Lemma mset_all_nil
-    :
-    ⊢ mset_all [].
-  Proof.
-    unfold mset_all. ss. auto.
-  Qed.
-
-  Lemma mset_all_cons_fold hd tl
-    :
-    (I hd ** mset_all tl)
-      -∗
-      (mset_all (hd::tl)).
-  Proof.
-    unfold mset_all. ss.
-  Qed.
-
-  Lemma mset_all_cons_unfold hd tl
-    :
-    (mset_all (hd::tl))
-      -∗
-      (I hd ** mset_all tl).
-  Proof.
-    unfold mset_all. ss.
-  Qed.
-
-  Lemma mset_all_split l0 l1
-    :
-    (mset_all (l0 ++ l1))
-      -∗
-      (mset_all l0 ** mset_all l1).
-  Proof.
-    induction l0; ss.
-    { iIntros "SAT". iFrame. }
-    { iIntros "[INTERP SAT]". iFrame. iApply IHl0; auto. }
-  Qed.
-
-  Lemma mset_all_combine l0 l1
-    :
-    (mset_all l0 ** mset_all l1)
-      -∗
-      (mset_all (l0 ++ l1)).
-  Proof.
-    induction l0; ss.
-    { iIntros "[_ SAT]". auto. }
-    { iIntros "[[INTERP SAT0] SAT1]". iFrame.
-      iApply IHl0. iFrame.
-    }
-  Qed.
-
-  Lemma mset_all_add l a
-    :
-    (I a ** mset_all l)
-      -∗
-      (mset_all (l++[a])).
-  Proof.
-    iIntros "[NEW SAT]". iApply mset_all_combine. iFrame.
-  Qed.
-
-  Lemma mset_all_permutation l0 l1
-        (PERM: Permutation l0 l1)
-    :
-    mset_all l0 ⊢ mset_all l1.
-  Proof.
-    induction PERM.
-    { auto. }
-    { iIntros "H". iApply mset_all_cons_fold.
-      iPoseProof (mset_all_cons_unfold with "H") as "[HD TL]".
-      iFrame. iApply IHPERM; auto.
-    }
-    { iIntros "H". iApply mset_all_cons_fold.
-      iPoseProof (mset_all_cons_unfold with "H") as "[HD0 TL]".
-      iPoseProof (mset_all_cons_unfold with "TL") as "[HD1 TL]".
-      iSplitL "HD1"; auto. iApply mset_all_cons_fold. iFrame.
-    }
-    { etrans; eauto. }
-  Qed.
-
-  Lemma mset_all_sub l0 l1
-        (SUB: mset_sub l0 l1)
-    :
-    mset_all l1 ⊢ mset_all l0 ** (mset_all l0 -* mset_all l1).
-  Proof.
-    rr in SUB. des. iIntros "H".
-    iPoseProof (mset_all_permutation with "H") as "H".
-    { symmetry. eauto. }
-    iPoseProof (mset_all_split with "H") as "[H0 H1]". iFrame.
-    iIntros "H1". iApply mset_all_permutation; eauto.
-    iApply mset_all_combine. iFrame.
-  Qed.
-
-  Lemma mset_all_discard l0 l1
-        (SUB: mset_sub l0 l1)
-    :
-    mset_all l1 ⊢ mset_all l0.
-  Proof.
-    rewrite mset_all_sub; eauto. iIntros "[H0 H1]". iFrame.
-  Qed.
-
-  Lemma mset_all_update l k a
-        (FIND: nth_error l k = Some a)
-    :
-    mset_all l ⊢ I a ** (I a -* mset_all l).
-  Proof.
-    hexploit nth_error_split; eauto. i. des. subst.
-    iIntros "SAT". iPoseProof (mset_all_split with "SAT") as "[SAT0 SAT1]".
-    iPoseProof (mset_all_cons_unfold with "SAT1") as "[OLD SAT1]".
-    iFrame. iIntros "NEW". iApply mset_all_combine. iFrame.
-  Qed.
-
-  Lemma mset_all_nth_sub l k a
-        (FIND: nth_error l k = Some a)
-    :
-    ⊢ SubIProp (I a) (mset_all l).
-  Proof.
-    iIntros "H". iPoseProof (mset_all_update with "H") as "[H0 H1]"; eauto.
-    iFrame. iModIntro. iIntros "H". iModIntro. iApply ("H1" with "H").
-  Qed.
-
-  Lemma list_remove_permutation A `{EqDecision A} a (l0 l1: list A)
-        (PERM: Permutation l0 l1)
-    :
-    option_Forall2 Permutation (list_remove a l0) (list_remove a l1).
-  Proof.
-    induction PERM; ss.
-    { econs. }
-    { des_ifs.
-      { econs. auto. }
-      { unfold fmap, option_fmap, option_map. inv IHPERM; econs.
-        econs. auto.
-      }
-    }
-    { des_ifs.
-      { econs. auto. }
-      { unfold fmap, option_fmap, option_map. reflexivity. }
-      { unfold fmap, option_fmap, option_map. reflexivity. }
-      { unfold fmap, option_fmap, option_map. des_ifs; econs. econs. }
-    }
-    { etrans; eauto. }
-  Qed.
-
-  Lemma list_remove_list_permutation_l A `{EqDecision A} (l l0 l1: list A)
-        (PERM: Permutation l0 l1)
-    :
-    option_Forall2 Permutation (list_remove_list l l0) (list_remove_list l l1).
-  Proof.
-    revert l0 l1 PERM. induction l; i.
-    { ss. econs; eauto. }
-    ss. unfold mbind, option_bind.
-    hexploit list_remove_permutation.
-    { eapply PERM. }
-    instantiate (1:=a). i. inv H.
-    { rewrite <- H0. rewrite <- H1. auto. }
-    { rewrite <- H1. rewrite <- H2. econs. }
-  Qed.
-
-  Lemma list_remove_add_permutation A `{EqDecision A} a (l0 l1: list A)
-        (REMOVE: list_remove a l0 = Some l1)
-    :
-    Permutation l0 (a :: l1).
-  Proof.
-    revert l1 REMOVE. induction l0; i; ss. des_ifs.
-    unfold fmap, option_fmap, option_map in REMOVE. des_ifs.
-    rewrite IHl0; eauto. econs.
-  Qed.
-
-  Lemma list_remove_list_add_permutation A `{EqDecision A} (l l0 l1: list A)
-        (REMOVE: list_remove_list l l0 = Some l1)
-    :
-    Permutation l0 (l ++ l1).
-  Proof.
-    revert l0 l1 REMOVE. induction l; i; ss.
-    { clarify. }
-    unfold mbind, option_bind in REMOVE. des_ifs.
-    hexploit IHl; eauto. i. rewrite <- H.
-    eapply list_remove_add_permutation; eauto.
-  Qed.
-
-  Lemma list_remove_list_permutation_r A `{EqDecision A} (l l0 l1: list A)
-        (PERM: Permutation l0 l1)
-    :
-    option_Forall2 Permutation (list_remove_list l0 l) (list_remove_list l1 l).
-  Proof.
-    destruct (list_remove_list l0 l) eqn:EQ0, (list_remove_list l1 l) eqn:EQ1.
-    { econs.
-      eapply list_remove_list_add_permutation in EQ0.
-      eapply list_remove_list_add_permutation in EQ1.
-      rewrite EQ0 in EQ1. rewrite PERM in EQ1.
-      eapply Permutation_app_inv_l; eauto.
-    }
-    { assert (submseteq l0 l).
-      { eapply list_remove_list_submseteq. rewrite EQ0. ss. }
-      rewrite PERM in H. eapply list_remove_list_submseteq in H.
-      rewrite EQ1 in H. inv H. ss.
-    }
-    { assert (submseteq l1 l).
-      { eapply list_remove_list_submseteq. rewrite EQ1. ss. }
-      rewrite <- PERM in H. eapply list_remove_list_submseteq in H.
-      rewrite EQ0 in H. inv H. ss.
-    }
-    { econs. }
-  Qed.
-
-  Global Instance permutation_mset_minus_proper:
-    Proper (Permutation ==> Permutation ==> Permutation) mset_minus.
-  Proof.
-    ii. unfold mset_minus.
-    cut (option_Forall2 Permutation (list_remove_list x0 x) (list_remove_list y0 y)).
-    { i. inv H1; ss. }
-    rewrite list_remove_list_permutation_r; [|eauto].
-    eapply list_remove_list_permutation_l; auto.
-  Qed.
-
-  Lemma mset_minus_add_eq E1 E
-        (SUB: mset_sub E1 E)
-    :
-    Permutation E (E1 ++ mset_minus E E1).
-  Proof.
-    rr in SUB. des. rewrite <- SUB.
-    unfold mset_minus.
-    assert (is_Some (list_remove_list E1 (s ++ E1))).
-    { eapply list_remove_list_submseteq.
-      eapply submseteq_inserts_l. reflexivity.
-    }
-    inv H. rewrite H0.
-    eapply list_remove_list_add_permutation; auto.
-  Qed.
-
-  Definition MUpd (l0 l1: mset) (P: iProp): iProp :=
-    (IA ** mset_all l0) -* #=> ((IA ** mset_all l1) ** P).
-
-  Lemma MUpd_open i:
-    ⊢ MUpd [i] [] (I i ** (I i -* (MUpd [] [i] True))).
-  Proof.
-    i. iIntros "[X [H0 H1]]". ss. iModIntro. iFrame.
-    iIntros "H0 [X H1]". iModIntro. ss. iFrame.
-  Qed.
-
-  Lemma MUpd_mask_subseteq E1 E2 :
-    mset_sub E2 E1 -> ⊢ MUpd E1 E2 (MUpd E2 E1 emp).
-  Proof.
-    i. iIntros "[X H]".
-    iPoseProof (mset_all_sub with "H") as "[H0 H1]"; eauto.
-    iModIntro. iFrame. iIntros "[X H0]". iModIntro. iSplit; auto. iFrame.
-    iApply "H1"; auto.
-  Qed.
-
-  Lemma MUpd_mono E1 E2 P Q
-    :
-    (P ⊢ Q) -> (MUpd E1 E2 P ⊢ MUpd E1 E2 Q).
-  Proof.
-    i. iIntros "H0 H1". iPoseProof ("H0" with "H1") as "> [H0 H1]".
-    iModIntro. iFrame. iApply H. auto.
-  Qed.
-
-  Lemma MUpd_trans E1 E2 E3 P
-    :
-    MUpd E1 E2 (MUpd E2 E3 P) ⊢ MUpd E1 E3 P.
-  Proof.
-    iIntros "H0 H1". iPoseProof ("H0" with "H1") as "> [H0 H1]".
-    iPoseProof ("H1" with "H0") as "> [H0 H1]".
-    iModIntro. iFrame.
-  Qed.
-
-  Lemma MUpd_frame_r E1 E2 P R
-    :
-    MUpd E1 E2 P ** R ⊢ MUpd E1 E2 (P ** R).
-  Proof.
-    iIntros "[H0 H1] H2". iPoseProof ("H0" with "H2") as "> [H0 H2]".
-    iModIntro. iFrame.
-  Qed.
-
-  Lemma MUpd_mask_frame_r E1 E2 Ef P
-    :
-    (MUpd E1 E2 P ⊢ MUpd (E1 ++ Ef) (E2 ++ Ef) P).
-  Proof.
-    i. iIntros "H0 [X H1]".
-    iPoseProof (mset_all_split with "H1") as "[H1 H2]".
-    iPoseProof ("H0" with "[X H1]") as "> [[X H0] H1]".
-    { iFrame. }
-    iModIntro. iFrame. iApply (mset_all_combine with "[H2 H0]"). iFrame.
-  Qed.
-
-  Global Instance MUpd_ne E1 E2 : NonExpansive (MUpd E1 E2).
-  Proof.
-    ii. unfold MUpd. rewrite H. auto.
-  Qed.
-
-  Global Instance MUpd_proper E1 E2 :
-    Proper ((≡) ==> (≡)) (MUpd E1 E2) := ne_proper _.
-
-  Global Instance MUpd_mono' E1 E2 : Proper ((⊢) ==> (⊢)) (MUpd E1 E2).
-  Proof. intros P Q; apply MUpd_mono. Qed.
-  Global Instance MUpd_flip_mono' E1 E2 :
-    Proper (flip (⊢) ==> flip (⊢)) (MUpd E1 E2).
-  Proof. intros P Q; apply MUpd_mono. Qed.
-
-  Lemma MUpd_mask_intro_subseteq E1 E2 P :
-    mset_sub E2 E1 -> P ⊢ MUpd E1 E2 (MUpd E2 E1 P).
-  Proof.
-    intros HE. iIntros "H0". iApply MUpd_mono.
-    { eapply MUpd_mono. instantiate (1:=emp ** P).
-      iIntros "[H0 H1]". auto.
-    }
-    { iApply MUpd_mono.
-      { iApply MUpd_frame_r. }
-      iApply MUpd_frame_r. iFrame.
-      iApply MUpd_mask_subseteq. auto.
-    }
-  Qed.
-
-  Lemma MUpd_intro E P : P ⊢ MUpd E E P.
-  Proof.
-    etrans.
-    { eapply MUpd_mask_intro_subseteq. reflexivity. }
-    { eapply MUpd_trans. }
-  Qed.
-
-  Lemma MUpd_idemp E P : (MUpd E E (MUpd E E P)) ⊣⊢ MUpd E E P.
-  Proof.
-    apply: anti_symm.
-    - apply MUpd_trans.
-    - apply MUpd_intro.
-  Qed.
-
-  Lemma MUpd_mask_weaken {E1} E2 {E3 P} :
-    mset_sub E2 E1 ->
-    (MUpd E2 E1 emp -* MUpd E2 E3 P) -∗ MUpd E1 E3 P.
-  Proof.
-    intros HE.
-    iIntros "H1".
-    iPoseProof MUpd_mask_subseteq as "H0"; eauto.
-    iPoseProof (MUpd_frame_r with "[H0 H1]") as "H".
-    { iSplitR "H1".
-      { iExact "H0". }
-      { iExact "H1". }
-    }
-    iApply MUpd_trans. iClear "H0".
-    iStopProof. eapply MUpd_mono.
-    eapply wand_elim_r.
-  Qed.
-
-  Lemma MUpd_mask_intro E1 E2 P :
-    mset_sub E2 E1 ->
-    ((MUpd E2 E1 emp) -∗ P) -∗ MUpd E1 E2 P.
-  Proof.
-    intros. etrans; [|by apply MUpd_mask_weaken].
-    rewrite <- MUpd_intro. auto.
-  Qed.
-
-  Lemma MUpd_mask_intro_discard E1 E2 P:
-    mset_sub E2 E1 -> P ⊢ MUpd E1 E2 P.
-  Proof.
-    intros. etrans; [|by apply MUpd_mask_intro].
-    apply Wand_intro_r. rewrite sep_elim_l; try done.
-    econs 2. typeclasses eauto.
-  Qed.
-
-  Lemma MUpd_frame_l E1 E2 R Q : (R ∗ MUpd E1 E2 Q) ⊢ MUpd E1 E2 (R ∗ Q).
-  Proof. rewrite !(comm _ R); apply MUpd_frame_r. Qed.
-  Lemma MUpd_wand_l E1 E2 P Q : (P -∗ Q) ∗ (MUpd E1 E2 P) ⊢ MUpd E1 E2 Q.
-  Proof. rewrite MUpd_frame_l. rewrite wand_elim_l. auto. Qed.
-  Lemma MUpd_wand_r E1 E2 P Q : (MUpd E1 E2 P) ∗ (P -∗ Q) ⊢ MUpd E1 E2 Q.
-  Proof. rewrite MUpd_frame_r. rewrite wand_elim_r. auto. Qed.
-
-  Lemma MUpd_trans_frame E1 E2 E3 P Q :
-    ((Q -* MUpd E2 E3 emp) ∗ MUpd E1 E2 (Q ∗ P)) ⊢ MUpd E1 E3 P.
-  Proof.
-    rewrite MUpd_frame_l.
-    iIntros "H0". iApply MUpd_trans.
-    iApply (MUpd_mono with "H0").
-    iIntros "[H0 [H1 H2]]".
-    iPoseProof ("H0" with "H1") as "H0".
-    iApply MUpd_mono.
-    { instantiate (1:=emp ** P). iIntros "[H0 H1]". auto. }
-    iApply MUpd_frame_r. iFrame.
-  Qed.
-
-  Lemma MUpd_elim E1 E2 E3 P Q :
-    (Q -∗ MUpd E2 E3 P) -> (MUpd E1 E2 Q) -∗ (MUpd E1 E3 P).
-  Proof.
-    i. rewrite H. rewrite MUpd_trans. auto.
-  Qed.
-
-  Lemma MUpd_permutation E1 E2 E1' E2' P
-        (PERM0: Permutation E1 E1')
-        (PERM1: Permutation E2 E2')
-    :
-    MUpd E1' E2' P ⊢ MUpd E1 E2 P.
-  Proof.
-    iIntros "H".
-    iApply MUpd_trans.
-    iApply MUpd_mask_intro_discard.
-    { rewrite PERM0. reflexivity. }
-    iApply MUpd_trans. iApply (MUpd_mono with "H").
-    iApply MUpd_mask_intro_discard. rewrite PERM1. reflexivity.
-  Qed.
-
-  Lemma MUpd_sort E1 E2 P
-    :
-    MUpd (NatSort.sort E1) (NatSort.sort E2) P ⊢ MUpd E1 E2 P.
-  Proof.
-    apply MUpd_permutation.
-    { apply Permuted_sort. }
-    { apply Permuted_sort. }
-  Qed.
-
-  Lemma MUpd_mask_mono E1 E2 P : mset_sub E1 E2 -> MUpd E1 E1 P ⊢ MUpd E2 E2 P.
-  Proof.
-    i. rr in H. des.
-    symmetry in H. rewrite Permutation_app_comm in H.
-    iIntros "H". iPoseProof (MUpd_mask_frame_r with "H") as "H".
-    iApply (MUpd_permutation with "H"); eauto.
-  Qed.
-
-  Lemma MUpd_mask_frame E E' E1 E2 P :
-    mset_sub E1 E →
-    (MUpd E1 E2 (MUpd (E2 ++ (mset_minus E E1)) E' P)) -∗ (MUpd E E' P).
-  Proof.
-    i. rewrite (MUpd_mask_frame_r _ _ (mset_minus E E1)).
-    rewrite MUpd_trans. eapply MUpd_permutation; eauto.
-    eapply mset_minus_add_eq. auto.
-  Qed.
-
-  Lemma MUpd_or E1 E2 P Q :
-    (MUpd E1 E2 P ∨ MUpd E1 E2 Q)
-      ⊢
-      (MUpd E1 E2 (P ∨ Q)).
-  Proof. apply Or_elim; apply MUpd_mono; [ apply Or_intro_l | apply Or_intro_r ]. Qed.
-
-  Global Instance MUpd_or_homomorphism E :
-    MonoidHomomorphism bi_or bi_or (flip (⊢)) (MUpd E E).
-  Proof. split; [split|]; try apply _; [apply MUpd_or | apply MUpd_intro]. Qed.
-
-  Lemma MUpd_and E1 E2 P Q :
-    (MUpd E1 E2 (P ∧ Q)) ⊢ (MUpd E1 E2 P) ∧ (MUpd E1 E2 Q).
-  Proof. apply And_intro; apply MUpd_mono; [apply And_elim_l | apply And_elim_r]. Qed.
-
-  Lemma MUpd_exist E1 E2 A (Φ : A → iProp) : (∃ x : A, MUpd E1 E2 (Φ x)) ⊢ MUpd E1 E2 (∃ x : A, Φ x).
-  Proof.
-    iIntros "[% H]". iApply (MUpd_mono with "H"). apply Ex_intro.
-  Qed.
-
-  Lemma MUpd_forall E1 E2 A (Φ : A → iProp) : (MUpd E1 E2 (∀ x : A, Φ x)) ⊢ ∀ x : A, MUpd E1 E2 (Φ x).
-  Proof.
-    iIntros "H %". iApply (MUpd_mono with "H"). apply Univ_elim.
-  Qed.
-
-  Lemma MUpd_sep E P Q : (MUpd E E P) ∗ (MUpd E E Q) ⊢ MUpd E E (P ∗ Q).
-  Proof. rewrite MUpd_frame_r. rewrite MUpd_frame_l. rewrite MUpd_trans. auto. Qed.
-
-  Global Instance MUpd_sep_homomorphism E :
-    MonoidHomomorphism bi_sep bi_sep (flip (⊢)) (MUpd E E).
-  Proof. split; [split|]; try apply _; [apply MUpd_sep | apply MUpd_intro]. Qed.
-
-  Lemma MUpd_mask_subseteq_emptyset_difference E1 E2 :
-    mset_sub E2 E1 ->
-    ⊢ MUpd E1 E2 (MUpd [] (mset_minus E1 E2) emp).
-  Proof.
-    i. iStartProof. iStopProof. etrans.
-    { eapply MUpd_mask_intro_subseteq.
-      instantiate (1:=mset_minus E1 E2). instantiate (1:=[]).
-      rr in H. rr. des.
-      exists s. rewrite app_nil_r. rewrite <- H.
-      eapply Permutation_app_inv_l. rewrite <- mset_minus_add_eq.
-      { apply Permutation_app_comm. }
-      { exists s. auto. }
-    }
-    etrans.
-    { eapply MUpd_mask_frame_r. }
-    eapply MUpd_permutation.
-    { instantiate (1:=E2). rewrite Permutation_app_comm. eapply mset_minus_add_eq. auto. }
-    { ss. }
-  Qed.
-
-  (* Lemma MUpd_mask_frame_acc E E' E1 E2 P Q : *)
-  (*   mset_sub E1 E -> *)
-  (*   (MUpd E1 (mset_minus E1 E2) Q) *)
-  (*     -∗ *)
-  (*     (Q -∗ MUpd (mset_minus E E2) E' (∀ R, MUpd (mset_minus E1 E2) E1 R -∗ MUpd (mset_minus E E2) E R) -∗ P) *)
-  (*     -∗ *)
-  (*     (MUpd E E' P). *)
-  (* Proof. *)
-  (*   intros HE. apply Wand_intro_r. rewrite MUpd_frame_r. *)
-  (*   rewrite wand_elim_r. clear Q. *)
-  (*   iIntros "H0". *)
-  (*   rewrite - (MUpd_mask_frame E E'). *)
-  (*   ; first apply fupd_mono; last done. *)
-  (*   (* The most horrible way to apply fupd_intro_mask *) *)
-  (*   rewrite -[X in (X -∗ _)](right_id emp%I). *)
-  (*   rewrite (fupd_mask_intro_subseteq (E1 ∖ E2 ∪ E ∖ E1) (E ∖ E2) emp%I); last first. *)
-  (*   { rewrite {1}(union_difference_L _ _ HE). set_solver. } *)
-  (*   rewrite fupd_frame_l fupd_frame_r. apply fupd_elim. *)
-  (*   apply fupd_mono. *)
-  (*   eapply wand_apply; *)
-  (*     last (apply sep_mono; first reflexivity); first reflexivity. *)
-  (*   apply forall_intro=>R. apply wand_intro_r. *)
-  (*   rewrite fupd_frame_r. apply fupd_elim. rewrite left_id. *)
-  (*   rewrite (fupd_mask_frame_r _ _ (E ∖ E1)); last set_solver+. *)
-  (*   rewrite {4}(union_difference_L _ _ HE). done. *)
-  (* Qed. *)
-
-  Lemma BUpd_MUpd E P:
-    #=> P ⊢ MUpd E E P.
-  Proof.
-    iIntros "H0 H1". iMod "H0". iModIntro. iFrame.
-  Qed.
-
-  Global Instance from_assumption_MUpd
-         E p P Q :
-    FromAssumption p P (#=> Q) → KnownRFromAssumption p P (MUpd E E Q).
-  Proof. rewrite /KnownRFromAssumption /FromAssumption=>->. apply BUpd_MUpd. Qed.
-
-  Global Instance from_pure_MUpd a E P φ :
-    FromPure a P φ → FromPure a (MUpd E E P) φ.
-  Proof. rewrite /FromPure=> <-. apply MUpd_intro. Qed.
-
-  Global Instance into_wand_MUpd E p q R P Q :
-    IntoWand false false R P Q →
-    IntoWand p q (MUpd E E R) (MUpd E E P) (MUpd E E Q).
-  Proof.
-    rewrite /IntoWand /= => HR. rewrite ! intuitionistically_if_elim.
-    rewrite ! HR. apply wand_intro_l. rewrite MUpd_sep. rewrite wand_elim_r. auto.
-  Qed.
-
-  Global Instance into_wand_MUpd_persistent E1 E2 p q R P Q :
-    IntoWand false q R P Q → IntoWand p q (MUpd E1 E2 R) P (MUpd E1 E2 Q).
-  Proof.
-    rewrite /IntoWand /= => HR. rewrite intuitionistically_if_elim. rewrite HR.
-    apply wand_intro_l. rewrite MUpd_frame_l. rewrite wand_elim_r. auto.
-  Qed.
-
-  Global Instance into_wand_MUpd_args E1 E2 p q R P Q :
-    IntoWand p false R P Q → IntoWand' p q R (MUpd E1 E2 P) (MUpd E1 E2 Q).
-  Proof.
-    rewrite /IntoWand' /IntoWand /= => ->.
-    apply wand_intro_l. rewrite intuitionistically_if_elim. rewrite MUpd_wand_r. auto.
-  Qed.
-
-  Global Instance from_sep_MUpd E P Q1 Q2 :
-    FromSep P Q1 Q2 → FromSep (MUpd E E P) (MUpd E E Q1) (MUpd E E Q2).
-  Proof. rewrite /FromSep =><-. apply MUpd_sep. Qed.
-
-  Global Instance from_or_MUpd E1 E2 P Q1 Q2 :
-    FromOr P Q1 Q2 → FromOr (MUpd E1 E2 P) (MUpd E1 E2 Q1) (MUpd E1 E2 Q2).
-  Proof. rewrite /FromOr=><-. apply MUpd_or. Qed.
-
-  Global Instance into_and_MUpd E1 E2 P Q1 Q2 :
-    IntoAnd false P Q1 Q2 → IntoAnd false (MUpd E1 E2 P) (MUpd E1 E2 Q1) (MUpd E1 E2 Q2).
-  Proof. rewrite /IntoAnd/==>->. apply MUpd_and. Qed.
-
-  Global Instance from_exist_MUpd {A} E1 E2 P (Φ : A → iProp) :
-    FromExist P Φ → FromExist (MUpd E1 E2 P) (λ a, MUpd E1 E2 (Φ a))%I.
-  Proof. rewrite /FromExist=><-. apply MUpd_exist. Qed.
-
-  Global Instance into_forall_MUpd {A} E1 E2 P (Φ : A → iProp) :
-    IntoForall P Φ → IntoForall (MUpd E1 E2 P) (λ a, MUpd E1 E2 (Φ a))%I.
-  Proof. rewrite /IntoForall=>->. apply MUpd_forall. Qed.
-
-  Global Instance from_modal_MUpd E P :
-    FromModal True modality_id (MUpd E E P) (MUpd E E P) P.
-  Proof. by rewrite /FromModal /= -MUpd_intro. Qed.
-
-  Global Instance from_modal_MUpd_wrong_mask E1 E2 P :
-    FromModal
-      (pm_error "Only non-mask-changing update modalities can be introduced directly.
-Use [iApply MUpd_mask_intro] to introduce mask-changing update modalities")
-      modality_id (MUpd E1 E2 P) (MUpd E1 E2 P) P | 100.
-  Proof. by intros []. Qed.
-
-  Global Instance elim_modal_bupd_MUpd
-         p E1 E2 P Q :
-    ElimModal True p false (|==> P) P (MUpd E1 E2 Q) (MUpd E1 E2 Q) | 10.
-  Proof.
-    unfold ElimModal. rewrite intuitionistically_if_elim.
-    rewrite (BUpd_MUpd E1). rewrite MUpd_frame_r. rewrite wand_elim_r. rewrite MUpd_trans. auto.
-  Qed.
-
-  Global Instance elim_modal_MUpd_MUpd_gen p E0 E1 E2 E3 P Q :
-    ElimModal (mset_sub E0 E2) p false (MUpd E0 E1 P) P (MUpd E2 E3 Q) (MUpd (E1 ++ mset_minus E2 E0) E3 Q).
-  Proof.
-    unfold ElimModal. i. rewrite intuitionistically_if_elim.
-    rewrite MUpd_frame_r. rewrite wand_elim_r. rewrite MUpd_mask_frame; eauto.
-  Qed.
-
-  Global Instance elim_modal_MUpd_MUpd p E1 E2 E3 P Q :
-    ElimModal True p false (MUpd E1 E2 P) P (MUpd E1 E3 Q) (MUpd E2 E3 Q).
-  Proof.
-    unfold ElimModal. rewrite intuitionistically_if_elim.
-    rewrite MUpd_frame_r. rewrite wand_elim_r. rewrite MUpd_trans. auto.
-  Qed.
-
-  Global Instance elim_modal_MUpd_MUpd_wrong_mask p E0 E1 E2 E3 P Q :
-    ElimModal
-      (pm_error "Goal and eliminated modality must have the same mask.
-Use [iMod (MUpd_mask_subseteq E2)] to adjust the mask of your goal to [E2]")
-      p false
-      (MUpd E1 E2 P) False (MUpd E0 E3 Q) False | 100.
-  Proof. intros []. Qed.
-
-  Global Instance add_modal_MUpd E1 E2 P Q :
-    AddModal (MUpd E1 E1 P) P (MUpd E1 E2 Q).
-  Proof.
-    unfold AddModal. rewrite MUpd_frame_r. rewrite wand_elim_r. rewrite MUpd_trans. auto.
-  Qed.
-
-  Global Instance elim_acc_MUpd {X} E1 E2 E α β mγ Q :
-    ElimAcc (X:=X) True (MUpd E1 E2) (MUpd E2 E1) α β mγ
-            (MUpd E1 E Q)
-            (λ x, MUpd E2 E2 (β x) ∗ (mγ x -∗? MUpd E1 E Q))%I.
-  Proof.
-    iIntros (_) "Hinner >Hacc". iDestruct "Hacc" as (x) "[Hα Hclose]".
-    iPoseProof ("Hinner" with "Hα") as "[> Hβ Hfin]".
-    iMod ("Hclose" with "Hβ") as "Hγ". by iApply "Hfin".
-  Qed.
-
-  Global Instance elim_modal_iupd_MUpd
-         p E1 E2 P Q :
-    ElimModal True p false (IUpd IA P) P (MUpd E1 E2 Q) (MUpd E1 E2 Q) | 10.
-  Proof.
-    unfold ElimModal. rewrite intuitionistically_if_elim.
-    i. iIntros "[H0 H1] [H2 H3]".
-    iPoseProof ("H0" with "H2") as "> [H2 H0]".
-    iApply ("H1" with "H0 [H2 H3]"). iFrame.
-  Qed.
-End MUPD.
-
-Ltac msubtac :=
-  try by (ss; apply mset_sub_b_reflect; ss).
-
-#[export] Hint Unfold NatSort.sort: mset.
-Ltac msimpl := autounfold with mset; simpl.
+(* Create HintDb mset. *)
+(* Section MUPD. *)
+(*   Definition mset := list nat. *)
+(*   Definition mset_disjoint (s0 s1: mset): Prop := *)
+(*     forall n (IN0: List.In n s0) (IN1: List.In n s1), False. *)
+
+(*   Fixpoint mset_disjoint_b (s0 s1: mset): bool := *)
+(*     match s0 with *)
+(*     | [] => true *)
+(*     | hd::tl => *)
+(*         match find (Nat.eqb hd) s1 with *)
+(*         | Some _ => false *)
+(*         | None => mset_disjoint_b tl s1 *)
+(*         end *)
+(*     end. *)
+
+(*   Lemma mset_disjoint_b_reflect s0 s1 *)
+(*     : *)
+(*     mset_disjoint s0 s1 <-> mset_disjoint_b s0 s1 = true. *)
+(*   Proof. *)
+(*     induction s0; ss. *)
+(*     { split; i; auto. ii. inv IN0. } *)
+(*     des_ifs. *)
+(*     { split; i. *)
+(*       { eapply find_some in Heq. des. *)
+(*         rewrite Nat.eqb_eq in Heq0. subst. *)
+(*         exfalso. eapply H; eauto. econs; ss. *)
+(*       } *)
+(*       { ii. inv IN0; eauto. } *)
+(*     } *)
+(*     { rewrite <- IHs0. split; i. *)
+(*       { ii. eapply H; eauto. econs 2; ss. } *)
+(*       { ii. inv IN0. *)
+(*         { eapply find_none in Heq; eauto. rewrite Nat.eqb_refl in Heq. ss. } *)
+(*         { eapply H; eauto. } *)
+(*       } *)
+(*     } *)
+(*   Qed. *)
+
+(*   Definition list_sub A (s0 s1: list A): Prop := *)
+(*     exists s, Permutation (s ++ s0) s1. *)
+
+(*   Global Program Instance list_sub_PreOrder A: PreOrder (@list_sub A). *)
+(*   Next Obligation. *)
+(*   Proof. *)
+(*     ii. exists []. ss. *)
+(*   Qed. *)
+(*   Next Obligation. *)
+(*   Proof. *)
+(*     ii. unfold list_sub in *. des. *)
+(*     rewrite <- H in H0. exists (s ++ s0). *)
+(*     rewrite <- app_assoc. auto. *)
+(*   Qed. *)
+
+(*   Global Instance permutation_list_sub_proper A: *)
+(*     Proper (Permutation ==> Permutation ==> iff) (@list_sub A). *)
+(*   Proof. *)
+(*     ii. unfold list_sub. split. *)
+(*     { i. des. exists s. rewrite <- H. rewrite H1. auto. } *)
+(*     { i. des. exists s. rewrite H0. rewrite H. auto. } *)
+(*   Qed. *)
+
+(*   Definition mset_sub (s0 s1: mset): Prop := list_sub s0 s1. *)
+
+(*   Global Program Instance mset_sub_PreOrder: PreOrder mset_sub. *)
+
+(*   Global Instance permutation_mset_sub_proper: *)
+(*     Proper (Permutation ==> Permutation ==> iff) mset_sub. *)
+(*   Proof. *)
+(*     unfold mset_sub. typeclasses eauto. *)
+(*   Qed. *)
+
+(*   Global Instance permutation_mset_disjoint_proper: *)
+(*     Proper (Permutation ==> Permutation ==> iff) mset_disjoint. *)
+(*   Proof. *)
+(*     ii. split. *)
+(*     { ii. eapply H1. *)
+(*       { symmetry in H. eapply Permutation_in; eauto. } *)
+(*       { symmetry in H0. eapply Permutation_in; eauto. } *)
+(*     } *)
+(*     { ii. eapply H1. *)
+(*       { eapply Permutation_in; eauto. } *)
+(*       { eapply Permutation_in; eauto. } *)
+(*     } *)
+(*   Qed. *)
+
+(*   Definition mset_minus (s0 s1: mset): mset := *)
+(*     match list_remove_list s1 s0 with *)
+(*     | Some s => s *)
+(*     | None => [] *)
+(*     end. *)
+
+(*   Definition mset_sub_b (s0 s1: mset): bool := *)
+(*     match list_remove_list s0 s1 with *)
+(*     | Some _ => true *)
+(*     | None => false *)
+(*     end. *)
+
+(*   Lemma list_remove_none A `{EqDecision A} (a: A) (l: list A) *)
+(*         (NONE: list_remove a l = None) *)
+(*     : *)
+(*     ~ List.In a l. *)
+(*   Proof. *)
+(*     revert NONE. induction l; ss. *)
+(*     des_ifs. i. unfold fmap, option_fmap, option_map in NONE. *)
+(*     des_ifs. ii. des; clarify. eapply IHl; auto. *)
+(*   Qed. *)
+
+(*   Lemma mset_sub_b_reflect s0 s1 *)
+(*     : *)
+(*     mset_sub s0 s1 <-> mset_sub_b s0 s1 = true. *)
+(*   Proof. *)
+(*     revert s1. induction s0; ss; i. *)
+(*     { split; i; auto. exists s1. rewrite app_nil_r. auto. } *)
+(*     { unfold mset_sub_b in *. ss. *)
+(*       destruct (list_remove a s1) eqn:EQ; ss. *)
+(*       { eapply list_remove_Some in EQ. *)
+(*         rewrite <- IHs0. unfold mset_sub, list_sub. split. *)
+(*         { i. des. rewrite EQ in H. *)
+(*           rewrite <- Permutation_middle in H. *)
+(*           apply Permutation_cons_inv in H. *)
+(*           exists s. auto. *)
+(*         } *)
+(*         { i. des. rewrite <- H in EQ. *)
+(*           eexists s. rewrite EQ. rewrite <- Permutation_middle. auto. *)
+(*         } *)
+(*       } *)
+(*       { eapply list_remove_none in EQ. split; i; ss. *)
+(*         exfalso. unfold mset_sub, list_sub in H. des. *)
+(*         rewrite <- Permutation_middle in H. *)
+(*         eapply EQ. eapply Permutation_in; eauto. *)
+(*         econs; ss. *)
+(*       } *)
+(*     } *)
+(*   Qed. *)
+
+(*   Context `{Σ: GRA.t}. *)
+(*   Variable I: nat -> iProp. *)
+(*   Variable IA: iProp. *)
+(*   Definition mset_all (l: mset) := fold_right (fun n P => I n ** P) True%I l. *)
+
+(*   Lemma mset_all_nil *)
+(*     : *)
+(*     ⊢ mset_all []. *)
+(*   Proof. *)
+(*     unfold mset_all. ss. auto. *)
+(*   Qed. *)
+
+(*   Lemma mset_all_cons_fold hd tl *)
+(*     : *)
+(*     (I hd ** mset_all tl) *)
+(*       -∗ *)
+(*       (mset_all (hd::tl)). *)
+(*   Proof. *)
+(*     unfold mset_all. ss. *)
+(*   Qed. *)
+
+(*   Lemma mset_all_cons_unfold hd tl *)
+(*     : *)
+(*     (mset_all (hd::tl)) *)
+(*       -∗ *)
+(*       (I hd ** mset_all tl). *)
+(*   Proof. *)
+(*     unfold mset_all. ss. *)
+(*   Qed. *)
+
+(*   Lemma mset_all_split l0 l1 *)
+(*     : *)
+(*     (mset_all (l0 ++ l1)) *)
+(*       -∗ *)
+(*       (mset_all l0 ** mset_all l1). *)
+(*   Proof. *)
+(*     induction l0; ss. *)
+(*     { iIntros "SAT". iFrame. } *)
+(*     { iIntros "[INTERP SAT]". iFrame. iApply IHl0; auto. } *)
+(*   Qed. *)
+
+(*   Lemma mset_all_combine l0 l1 *)
+(*     : *)
+(*     (mset_all l0 ** mset_all l1) *)
+(*       -∗ *)
+(*       (mset_all (l0 ++ l1)). *)
+(*   Proof. *)
+(*     induction l0; ss. *)
+(*     { iIntros "[_ SAT]". auto. } *)
+(*     { iIntros "[[INTERP SAT0] SAT1]". iFrame. *)
+(*       iApply IHl0. iFrame. *)
+(*     } *)
+(*   Qed. *)
+
+(*   Lemma mset_all_add l a *)
+(*     : *)
+(*     (I a ** mset_all l) *)
+(*       -∗ *)
+(*       (mset_all (l++[a])). *)
+(*   Proof. *)
+(*     iIntros "[NEW SAT]". iApply mset_all_combine. iFrame. *)
+(*   Qed. *)
+
+(*   Lemma mset_all_permutation l0 l1 *)
+(*         (PERM: Permutation l0 l1) *)
+(*     : *)
+(*     mset_all l0 ⊢ mset_all l1. *)
+(*   Proof. *)
+(*     induction PERM. *)
+(*     { auto. } *)
+(*     { iIntros "H". iApply mset_all_cons_fold. *)
+(*       iPoseProof (mset_all_cons_unfold with "H") as "[HD TL]". *)
+(*       iFrame. iApply IHPERM; auto. *)
+(*     } *)
+(*     { iIntros "H". iApply mset_all_cons_fold. *)
+(*       iPoseProof (mset_all_cons_unfold with "H") as "[HD0 TL]". *)
+(*       iPoseProof (mset_all_cons_unfold with "TL") as "[HD1 TL]". *)
+(*       iSplitL "HD1"; auto. iApply mset_all_cons_fold. iFrame. *)
+(*     } *)
+(*     { etrans; eauto. } *)
+(*   Qed. *)
+
+(*   Lemma mset_all_sub l0 l1 *)
+(*         (SUB: mset_sub l0 l1) *)
+(*     : *)
+(*     mset_all l1 ⊢ mset_all l0 ** (mset_all l0 -* mset_all l1). *)
+(*   Proof. *)
+(*     rr in SUB. des. iIntros "H". *)
+(*     iPoseProof (mset_all_permutation with "H") as "H". *)
+(*     { symmetry. eauto. } *)
+(*     iPoseProof (mset_all_split with "H") as "[H0 H1]". iFrame. *)
+(*     iIntros "H1". iApply mset_all_permutation; eauto. *)
+(*     iApply mset_all_combine. iFrame. *)
+(*   Qed. *)
+
+(*   Lemma mset_all_discard l0 l1 *)
+(*         (SUB: mset_sub l0 l1) *)
+(*     : *)
+(*     mset_all l1 ⊢ mset_all l0. *)
+(*   Proof. *)
+(*     rewrite mset_all_sub; eauto. iIntros "[H0 H1]". iFrame. *)
+(*   Qed. *)
+
+(*   Lemma mset_all_update l k a *)
+(*         (FIND: nth_error l k = Some a) *)
+(*     : *)
+(*     mset_all l ⊢ I a ** (I a -* mset_all l). *)
+(*   Proof. *)
+(*     hexploit nth_error_split; eauto. i. des. subst. *)
+(*     iIntros "SAT". iPoseProof (mset_all_split with "SAT") as "[SAT0 SAT1]". *)
+(*     iPoseProof (mset_all_cons_unfold with "SAT1") as "[OLD SAT1]". *)
+(*     iFrame. iIntros "NEW". iApply mset_all_combine. iFrame. *)
+(*   Qed. *)
+
+(*   Lemma mset_all_nth_sub l k a *)
+(*         (FIND: nth_error l k = Some a) *)
+(*     : *)
+(*     ⊢ SubIProp (I a) (mset_all l). *)
+(*   Proof. *)
+(*     iIntros "H". iPoseProof (mset_all_update with "H") as "[H0 H1]"; eauto. *)
+(*     iFrame. iModIntro. iIntros "H". iModIntro. iApply ("H1" with "H"). *)
+(*   Qed. *)
+
+(*   Lemma list_remove_permutation A `{EqDecision A} a (l0 l1: list A) *)
+(*         (PERM: Permutation l0 l1) *)
+(*     : *)
+(*     option_Forall2 Permutation (list_remove a l0) (list_remove a l1). *)
+(*   Proof. *)
+(*     induction PERM; ss. *)
+(*     { econs. } *)
+(*     { des_ifs. *)
+(*       { econs. auto. } *)
+(*       { unfold fmap, option_fmap, option_map. inv IHPERM; econs. *)
+(*         econs. auto. *)
+(*       } *)
+(*     } *)
+(*     { des_ifs. *)
+(*       { econs. auto. } *)
+(*       { unfold fmap, option_fmap, option_map. reflexivity. } *)
+(*       { unfold fmap, option_fmap, option_map. reflexivity. } *)
+(*       { unfold fmap, option_fmap, option_map. des_ifs; econs. econs. } *)
+(*     } *)
+(*     { etrans; eauto. } *)
+(*   Qed. *)
+
+(*   Lemma list_remove_list_permutation_l A `{EqDecision A} (l l0 l1: list A) *)
+(*         (PERM: Permutation l0 l1) *)
+(*     : *)
+(*     option_Forall2 Permutation (list_remove_list l l0) (list_remove_list l l1). *)
+(*   Proof. *)
+(*     revert l0 l1 PERM. induction l; i. *)
+(*     { ss. econs; eauto. } *)
+(*     ss. unfold mbind, option_bind. *)
+(*     hexploit list_remove_permutation. *)
+(*     { eapply PERM. } *)
+(*     instantiate (1:=a). i. inv H. *)
+(*     { rewrite <- H0. rewrite <- H1. auto. } *)
+(*     { rewrite <- H1. rewrite <- H2. econs. } *)
+(*   Qed. *)
+
+(*   Lemma list_remove_add_permutation A `{EqDecision A} a (l0 l1: list A) *)
+(*         (REMOVE: list_remove a l0 = Some l1) *)
+(*     : *)
+(*     Permutation l0 (a :: l1). *)
+(*   Proof. *)
+(*     revert l1 REMOVE. induction l0; i; ss. des_ifs. *)
+(*     unfold fmap, option_fmap, option_map in REMOVE. des_ifs. *)
+(*     rewrite IHl0; eauto. econs. *)
+(*   Qed. *)
+
+(*   Lemma list_remove_list_add_permutation A `{EqDecision A} (l l0 l1: list A) *)
+(*         (REMOVE: list_remove_list l l0 = Some l1) *)
+(*     : *)
+(*     Permutation l0 (l ++ l1). *)
+(*   Proof. *)
+(*     revert l0 l1 REMOVE. induction l; i; ss. *)
+(*     { clarify. } *)
+(*     unfold mbind, option_bind in REMOVE. des_ifs. *)
+(*     hexploit IHl; eauto. i. rewrite <- H. *)
+(*     eapply list_remove_add_permutation; eauto. *)
+(*   Qed. *)
+
+(*   Lemma list_remove_list_permutation_r A `{EqDecision A} (l l0 l1: list A) *)
+(*         (PERM: Permutation l0 l1) *)
+(*     : *)
+(*     option_Forall2 Permutation (list_remove_list l0 l) (list_remove_list l1 l). *)
+(*   Proof. *)
+(*     destruct (list_remove_list l0 l) eqn:EQ0, (list_remove_list l1 l) eqn:EQ1. *)
+(*     { econs. *)
+(*       eapply list_remove_list_add_permutation in EQ0. *)
+(*       eapply list_remove_list_add_permutation in EQ1. *)
+(*       rewrite EQ0 in EQ1. rewrite PERM in EQ1. *)
+(*       eapply Permutation_app_inv_l; eauto. *)
+(*     } *)
+(*     { assert (submseteq l0 l). *)
+(*       { eapply list_remove_list_submseteq. rewrite EQ0. ss. } *)
+(*       rewrite PERM in H. eapply list_remove_list_submseteq in H. *)
+(*       rewrite EQ1 in H. inv H. ss. *)
+(*     } *)
+(*     { assert (submseteq l1 l). *)
+(*       { eapply list_remove_list_submseteq. rewrite EQ1. ss. } *)
+(*       rewrite <- PERM in H. eapply list_remove_list_submseteq in H. *)
+(*       rewrite EQ0 in H. inv H. ss. *)
+(*     } *)
+(*     { econs. } *)
+(*   Qed. *)
+
+(*   Global Instance permutation_mset_minus_proper: *)
+(*     Proper (Permutation ==> Permutation ==> Permutation) mset_minus. *)
+(*   Proof. *)
+(*     ii. unfold mset_minus. *)
+(*     cut (option_Forall2 Permutation (list_remove_list x0 x) (list_remove_list y0 y)). *)
+(*     { i. inv H1; ss. } *)
+(*     rewrite list_remove_list_permutation_r; [|eauto]. *)
+(*     eapply list_remove_list_permutation_l; auto. *)
+(*   Qed. *)
+
+(*   Lemma mset_minus_add_eq E1 E *)
+(*         (SUB: mset_sub E1 E) *)
+(*     : *)
+(*     Permutation E (E1 ++ mset_minus E E1). *)
+(*   Proof. *)
+(*     rr in SUB. des. rewrite <- SUB. *)
+(*     unfold mset_minus. *)
+(*     assert (is_Some (list_remove_list E1 (s ++ E1))). *)
+(*     { eapply list_remove_list_submseteq. *)
+(*       eapply submseteq_inserts_l. reflexivity. *)
+(*     } *)
+(*     inv H. rewrite H0. *)
+(*     eapply list_remove_list_add_permutation; auto. *)
+(*   Qed. *)
+
+(*   Definition MUpd (l0 l1: mset) (P: iProp): iProp := *)
+(*     (IA ** mset_all l0) -* #=> ((IA ** mset_all l1) ** P). *)
+
+(*   Lemma MUpd_open i: *)
+(*     ⊢ MUpd [i] [] (I i ** (I i -* (MUpd [] [i] True))). *)
+(*   Proof. *)
+(*     i. iIntros "[X [H0 H1]]". ss. iModIntro. iFrame. *)
+(*     iIntros "H0 [X H1]". iModIntro. ss. iFrame. *)
+(*   Qed. *)
+
+(*   Lemma MUpd_mask_subseteq E1 E2 : *)
+(*     mset_sub E2 E1 -> ⊢ MUpd E1 E2 (MUpd E2 E1 emp). *)
+(*   Proof. *)
+(*     i. iIntros "[X H]". *)
+(*     iPoseProof (mset_all_sub with "H") as "[H0 H1]"; eauto. *)
+(*     iModIntro. iFrame. iIntros "[X H0]". iModIntro. iSplit; auto. iFrame. *)
+(*     iApply "H1"; auto. *)
+(*   Qed. *)
+
+(*   Lemma MUpd_mono E1 E2 P Q *)
+(*     : *)
+(*     (P ⊢ Q) -> (MUpd E1 E2 P ⊢ MUpd E1 E2 Q). *)
+(*   Proof. *)
+(*     i. iIntros "H0 H1". iPoseProof ("H0" with "H1") as "> [H0 H1]". *)
+(*     iModIntro. iFrame. iApply H. auto. *)
+(*   Qed. *)
+
+(*   Lemma MUpd_trans E1 E2 E3 P *)
+(*     : *)
+(*     MUpd E1 E2 (MUpd E2 E3 P) ⊢ MUpd E1 E3 P. *)
+(*   Proof. *)
+(*     iIntros "H0 H1". iPoseProof ("H0" with "H1") as "> [H0 H1]". *)
+(*     iPoseProof ("H1" with "H0") as "> [H0 H1]". *)
+(*     iModIntro. iFrame. *)
+(*   Qed. *)
+
+(*   Lemma MUpd_frame_r E1 E2 P R *)
+(*     : *)
+(*     MUpd E1 E2 P ** R ⊢ MUpd E1 E2 (P ** R). *)
+(*   Proof. *)
+(*     iIntros "[H0 H1] H2". iPoseProof ("H0" with "H2") as "> [H0 H2]". *)
+(*     iModIntro. iFrame. *)
+(*   Qed. *)
+
+(*   Lemma MUpd_mask_frame_r E1 E2 Ef P *)
+(*     : *)
+(*     (MUpd E1 E2 P ⊢ MUpd (E1 ++ Ef) (E2 ++ Ef) P). *)
+(*   Proof. *)
+(*     i. iIntros "H0 [X H1]". *)
+(*     iPoseProof (mset_all_split with "H1") as "[H1 H2]". *)
+(*     iPoseProof ("H0" with "[X H1]") as "> [[X H0] H1]". *)
+(*     { iFrame. } *)
+(*     iModIntro. iFrame. iApply (mset_all_combine with "[H2 H0]"). iFrame. *)
+(*   Qed. *)
+
+(*   Global Instance MUpd_ne E1 E2 : NonExpansive (MUpd E1 E2). *)
+(*   Proof. *)
+(*     ii. unfold MUpd. rewrite H. auto. *)
+(*   Qed. *)
+
+(*   Global Instance MUpd_proper E1 E2 : *)
+(*     Proper ((≡) ==> (≡)) (MUpd E1 E2) := ne_proper _. *)
+
+(*   Global Instance MUpd_mono' E1 E2 : Proper ((⊢) ==> (⊢)) (MUpd E1 E2). *)
+(*   Proof. intros P Q; apply MUpd_mono. Qed. *)
+(*   Global Instance MUpd_flip_mono' E1 E2 : *)
+(*     Proper (flip (⊢) ==> flip (⊢)) (MUpd E1 E2). *)
+(*   Proof. intros P Q; apply MUpd_mono. Qed. *)
+
+(*   Lemma MUpd_mask_intro_subseteq E1 E2 P : *)
+(*     mset_sub E2 E1 -> P ⊢ MUpd E1 E2 (MUpd E2 E1 P). *)
+(*   Proof. *)
+(*     intros HE. iIntros "H0". iApply MUpd_mono. *)
+(*     { eapply MUpd_mono. instantiate (1:=emp ** P). *)
+(*       iIntros "[H0 H1]". auto. *)
+(*     } *)
+(*     { iApply MUpd_mono. *)
+(*       { iApply MUpd_frame_r. } *)
+(*       iApply MUpd_frame_r. iFrame. *)
+(*       iApply MUpd_mask_subseteq. auto. *)
+(*     } *)
+(*   Qed. *)
+
+(*   Lemma MUpd_intro E P : P ⊢ MUpd E E P. *)
+(*   Proof. *)
+(*     etrans. *)
+(*     { eapply MUpd_mask_intro_subseteq. reflexivity. } *)
+(*     { eapply MUpd_trans. } *)
+(*   Qed. *)
+
+(*   Lemma MUpd_idemp E P : (MUpd E E (MUpd E E P)) ⊣⊢ MUpd E E P. *)
+(*   Proof. *)
+(*     apply: anti_symm. *)
+(*     - apply MUpd_trans. *)
+(*     - apply MUpd_intro. *)
+(*   Qed. *)
+
+(*   Lemma MUpd_mask_weaken {E1} E2 {E3 P} : *)
+(*     mset_sub E2 E1 -> *)
+(*     (MUpd E2 E1 emp -* MUpd E2 E3 P) -∗ MUpd E1 E3 P. *)
+(*   Proof. *)
+(*     intros HE. *)
+(*     iIntros "H1". *)
+(*     iPoseProof MUpd_mask_subseteq as "H0"; eauto. *)
+(*     iPoseProof (MUpd_frame_r with "[H0 H1]") as "H". *)
+(*     { iSplitR "H1". *)
+(*       { iExact "H0". } *)
+(*       { iExact "H1". } *)
+(*     } *)
+(*     iApply MUpd_trans. iClear "H0". *)
+(*     iStopProof. eapply MUpd_mono. *)
+(*     eapply wand_elim_r. *)
+(*   Qed. *)
+
+(*   Lemma MUpd_mask_intro E1 E2 P : *)
+(*     mset_sub E2 E1 -> *)
+(*     ((MUpd E2 E1 emp) -∗ P) -∗ MUpd E1 E2 P. *)
+(*   Proof. *)
+(*     intros. etrans; [|by apply MUpd_mask_weaken]. *)
+(*     rewrite <- MUpd_intro. auto. *)
+(*   Qed. *)
+
+(*   Lemma MUpd_mask_intro_discard E1 E2 P: *)
+(*     mset_sub E2 E1 -> P ⊢ MUpd E1 E2 P. *)
+(*   Proof. *)
+(*     intros. etrans; [|by apply MUpd_mask_intro]. *)
+(*     apply Wand_intro_r. rewrite sep_elim_l; try done. *)
+(*     econs 2. typeclasses eauto. *)
+(*   Qed. *)
+
+(*   Lemma MUpd_frame_l E1 E2 R Q : (R ∗ MUpd E1 E2 Q) ⊢ MUpd E1 E2 (R ∗ Q). *)
+(*   Proof. rewrite !(comm _ R); apply MUpd_frame_r. Qed. *)
+(*   Lemma MUpd_wand_l E1 E2 P Q : (P -∗ Q) ∗ (MUpd E1 E2 P) ⊢ MUpd E1 E2 Q. *)
+(*   Proof. rewrite MUpd_frame_l. rewrite wand_elim_l. auto. Qed. *)
+(*   Lemma MUpd_wand_r E1 E2 P Q : (MUpd E1 E2 P) ∗ (P -∗ Q) ⊢ MUpd E1 E2 Q. *)
+(*   Proof. rewrite MUpd_frame_r. rewrite wand_elim_r. auto. Qed. *)
+
+(*   Lemma MUpd_trans_frame E1 E2 E3 P Q : *)
+(*     ((Q -* MUpd E2 E3 emp) ∗ MUpd E1 E2 (Q ∗ P)) ⊢ MUpd E1 E3 P. *)
+(*   Proof. *)
+(*     rewrite MUpd_frame_l. *)
+(*     iIntros "H0". iApply MUpd_trans. *)
+(*     iApply (MUpd_mono with "H0"). *)
+(*     iIntros "[H0 [H1 H2]]". *)
+(*     iPoseProof ("H0" with "H1") as "H0". *)
+(*     iApply MUpd_mono. *)
+(*     { instantiate (1:=emp ** P). iIntros "[H0 H1]". auto. } *)
+(*     iApply MUpd_frame_r. iFrame. *)
+(*   Qed. *)
+
+(*   Lemma MUpd_elim E1 E2 E3 P Q : *)
+(*     (Q -∗ MUpd E2 E3 P) -> (MUpd E1 E2 Q) -∗ (MUpd E1 E3 P). *)
+(*   Proof. *)
+(*     i. rewrite H. rewrite MUpd_trans. auto. *)
+(*   Qed. *)
+
+(*   Lemma MUpd_permutation E1 E2 E1' E2' P *)
+(*         (PERM0: Permutation E1 E1') *)
+(*         (PERM1: Permutation E2 E2') *)
+(*     : *)
+(*     MUpd E1' E2' P ⊢ MUpd E1 E2 P. *)
+(*   Proof. *)
+(*     iIntros "H". *)
+(*     iApply MUpd_trans. *)
+(*     iApply MUpd_mask_intro_discard. *)
+(*     { rewrite PERM0. reflexivity. } *)
+(*     iApply MUpd_trans. iApply (MUpd_mono with "H"). *)
+(*     iApply MUpd_mask_intro_discard. rewrite PERM1. reflexivity. *)
+(*   Qed. *)
+
+(*   Lemma MUpd_sort E1 E2 P *)
+(*     : *)
+(*     MUpd (NatSort.sort E1) (NatSort.sort E2) P ⊢ MUpd E1 E2 P. *)
+(*   Proof. *)
+(*     apply MUpd_permutation. *)
+(*     { apply Permuted_sort. } *)
+(*     { apply Permuted_sort. } *)
+(*   Qed. *)
+
+(*   Lemma MUpd_mask_mono E1 E2 P : mset_sub E1 E2 -> MUpd E1 E1 P ⊢ MUpd E2 E2 P. *)
+(*   Proof. *)
+(*     i. rr in H. des. *)
+(*     symmetry in H. rewrite Permutation_app_comm in H. *)
+(*     iIntros "H". iPoseProof (MUpd_mask_frame_r with "H") as "H". *)
+(*     iApply (MUpd_permutation with "H"); eauto. *)
+(*   Qed. *)
+
+(*   Lemma MUpd_mask_frame E E' E1 E2 P : *)
+(*     mset_sub E1 E → *)
+(*     (MUpd E1 E2 (MUpd (E2 ++ (mset_minus E E1)) E' P)) -∗ (MUpd E E' P). *)
+(*   Proof. *)
+(*     i. rewrite (MUpd_mask_frame_r _ _ (mset_minus E E1)). *)
+(*     rewrite MUpd_trans. eapply MUpd_permutation; eauto. *)
+(*     eapply mset_minus_add_eq. auto. *)
+(*   Qed. *)
+
+(*   Lemma MUpd_or E1 E2 P Q : *)
+(*     (MUpd E1 E2 P ∨ MUpd E1 E2 Q) *)
+(*       ⊢ *)
+(*       (MUpd E1 E2 (P ∨ Q)). *)
+(*   Proof. apply Or_elim; apply MUpd_mono; [ apply Or_intro_l | apply Or_intro_r ]. Qed. *)
+
+(*   Global Instance MUpd_or_homomorphism E : *)
+(*     MonoidHomomorphism bi_or bi_or (flip (⊢)) (MUpd E E). *)
+(*   Proof. split; [split|]; try apply _; [apply MUpd_or | apply MUpd_intro]. Qed. *)
+
+(*   Lemma MUpd_and E1 E2 P Q : *)
+(*     (MUpd E1 E2 (P ∧ Q)) ⊢ (MUpd E1 E2 P) ∧ (MUpd E1 E2 Q). *)
+(*   Proof. apply And_intro; apply MUpd_mono; [apply And_elim_l | apply And_elim_r]. Qed. *)
+
+(*   Lemma MUpd_exist E1 E2 A (Φ : A → iProp) : (∃ x : A, MUpd E1 E2 (Φ x)) ⊢ MUpd E1 E2 (∃ x : A, Φ x). *)
+(*   Proof. *)
+(*     iIntros "[% H]". iApply (MUpd_mono with "H"). apply Ex_intro. *)
+(*   Qed. *)
+
+(*   Lemma MUpd_forall E1 E2 A (Φ : A → iProp) : (MUpd E1 E2 (∀ x : A, Φ x)) ⊢ ∀ x : A, MUpd E1 E2 (Φ x). *)
+(*   Proof. *)
+(*     iIntros "H %". iApply (MUpd_mono with "H"). apply Univ_elim. *)
+(*   Qed. *)
+
+(*   Lemma MUpd_sep E P Q : (MUpd E E P) ∗ (MUpd E E Q) ⊢ MUpd E E (P ∗ Q). *)
+(*   Proof. rewrite MUpd_frame_r. rewrite MUpd_frame_l. rewrite MUpd_trans. auto. Qed. *)
+
+(*   Global Instance MUpd_sep_homomorphism E : *)
+(*     MonoidHomomorphism bi_sep bi_sep (flip (⊢)) (MUpd E E). *)
+(*   Proof. split; [split|]; try apply _; [apply MUpd_sep | apply MUpd_intro]. Qed. *)
+
+(*   Lemma MUpd_mask_subseteq_emptyset_difference E1 E2 : *)
+(*     mset_sub E2 E1 -> *)
+(*     ⊢ MUpd E1 E2 (MUpd [] (mset_minus E1 E2) emp). *)
+(*   Proof. *)
+(*     i. iStartProof. iStopProof. etrans. *)
+(*     { eapply MUpd_mask_intro_subseteq. *)
+(*       instantiate (1:=mset_minus E1 E2). instantiate (1:=[]). *)
+(*       rr in H. rr. des. *)
+(*       exists s. rewrite app_nil_r. rewrite <- H. *)
+(*       eapply Permutation_app_inv_l. rewrite <- mset_minus_add_eq. *)
+(*       { apply Permutation_app_comm. } *)
+(*       { exists s. auto. } *)
+(*     } *)
+(*     etrans. *)
+(*     { eapply MUpd_mask_frame_r. } *)
+(*     eapply MUpd_permutation. *)
+(*     { instantiate (1:=E2). rewrite Permutation_app_comm. eapply mset_minus_add_eq. auto. } *)
+(*     { ss. } *)
+(*   Qed. *)
+
+(*   (* Lemma MUpd_mask_frame_acc E E' E1 E2 P Q : *) *)
+(*   (*   mset_sub E1 E -> *) *)
+(*   (*   (MUpd E1 (mset_minus E1 E2) Q) *) *)
+(*   (*     -∗ *) *)
+(*   (*     (Q -∗ MUpd (mset_minus E E2) E' (∀ R, MUpd (mset_minus E1 E2) E1 R -∗ MUpd (mset_minus E E2) E R) -∗ P) *) *)
+(*   (*     -∗ *) *)
+(*   (*     (MUpd E E' P). *) *)
+(*   (* Proof. *) *)
+(*   (*   intros HE. apply Wand_intro_r. rewrite MUpd_frame_r. *) *)
+(*   (*   rewrite wand_elim_r. clear Q. *) *)
+(*   (*   iIntros "H0". *) *)
+(*   (*   rewrite - (MUpd_mask_frame E E'). *) *)
+(*   (*   ; first apply fupd_mono; last done. *) *)
+(*   (*   (* The most horrible way to apply fupd_intro_mask *) *) *)
+(*   (*   rewrite -[X in (X -∗ _)](right_id emp%I). *) *)
+(*   (*   rewrite (fupd_mask_intro_subseteq (E1 ∖ E2 ∪ E ∖ E1) (E ∖ E2) emp%I); last first. *) *)
+(*   (*   { rewrite {1}(union_difference_L _ _ HE). set_solver. } *) *)
+(*   (*   rewrite fupd_frame_l fupd_frame_r. apply fupd_elim. *) *)
+(*   (*   apply fupd_mono. *) *)
+(*   (*   eapply wand_apply; *) *)
+(*   (*     last (apply sep_mono; first reflexivity); first reflexivity. *) *)
+(*   (*   apply forall_intro=>R. apply wand_intro_r. *) *)
+(*   (*   rewrite fupd_frame_r. apply fupd_elim. rewrite left_id. *) *)
+(*   (*   rewrite (fupd_mask_frame_r _ _ (E ∖ E1)); last set_solver+. *) *)
+(*   (*   rewrite {4}(union_difference_L _ _ HE). done. *) *)
+(*   (* Qed. *) *)
+
+(*   Lemma BUpd_MUpd E P: *)
+(*     #=> P ⊢ MUpd E E P. *)
+(*   Proof. *)
+(*     iIntros "H0 H1". iMod "H0". iModIntro. iFrame. *)
+(*   Qed. *)
+
+(*   Global Instance from_assumption_MUpd *)
+(*          E p P Q : *)
+(*     FromAssumption p P (#=> Q) → KnownRFromAssumption p P (MUpd E E Q). *)
+(*   Proof. rewrite /KnownRFromAssumption /FromAssumption=>->. apply BUpd_MUpd. Qed. *)
+
+(*   Global Instance from_pure_MUpd a E P φ : *)
+(*     FromPure a P φ → FromPure a (MUpd E E P) φ. *)
+(*   Proof. rewrite /FromPure=> <-. apply MUpd_intro. Qed. *)
+
+(*   Global Instance into_wand_MUpd E p q R P Q : *)
+(*     IntoWand false false R P Q → *)
+(*     IntoWand p q (MUpd E E R) (MUpd E E P) (MUpd E E Q). *)
+(*   Proof. *)
+(*     rewrite /IntoWand /= => HR. rewrite ! intuitionistically_if_elim. *)
+(*     rewrite ! HR. apply wand_intro_l. rewrite MUpd_sep. rewrite wand_elim_r. auto. *)
+(*   Qed. *)
+
+(*   Global Instance into_wand_MUpd_persistent E1 E2 p q R P Q : *)
+(*     IntoWand false q R P Q → IntoWand p q (MUpd E1 E2 R) P (MUpd E1 E2 Q). *)
+(*   Proof. *)
+(*     rewrite /IntoWand /= => HR. rewrite intuitionistically_if_elim. rewrite HR. *)
+(*     apply wand_intro_l. rewrite MUpd_frame_l. rewrite wand_elim_r. auto. *)
+(*   Qed. *)
+
+(*   Global Instance into_wand_MUpd_args E1 E2 p q R P Q : *)
+(*     IntoWand p false R P Q → IntoWand' p q R (MUpd E1 E2 P) (MUpd E1 E2 Q). *)
+(*   Proof. *)
+(*     rewrite /IntoWand' /IntoWand /= => ->. *)
+(*     apply wand_intro_l. rewrite intuitionistically_if_elim. rewrite MUpd_wand_r. auto. *)
+(*   Qed. *)
+
+(*   Global Instance from_sep_MUpd E P Q1 Q2 : *)
+(*     FromSep P Q1 Q2 → FromSep (MUpd E E P) (MUpd E E Q1) (MUpd E E Q2). *)
+(*   Proof. rewrite /FromSep =><-. apply MUpd_sep. Qed. *)
+
+(*   Global Instance from_or_MUpd E1 E2 P Q1 Q2 : *)
+(*     FromOr P Q1 Q2 → FromOr (MUpd E1 E2 P) (MUpd E1 E2 Q1) (MUpd E1 E2 Q2). *)
+(*   Proof. rewrite /FromOr=><-. apply MUpd_or. Qed. *)
+
+(*   Global Instance into_and_MUpd E1 E2 P Q1 Q2 : *)
+(*     IntoAnd false P Q1 Q2 → IntoAnd false (MUpd E1 E2 P) (MUpd E1 E2 Q1) (MUpd E1 E2 Q2). *)
+(*   Proof. rewrite /IntoAnd/==>->. apply MUpd_and. Qed. *)
+
+(*   Global Instance from_exist_MUpd {A} E1 E2 P (Φ : A → iProp) : *)
+(*     FromExist P Φ → FromExist (MUpd E1 E2 P) (λ a, MUpd E1 E2 (Φ a))%I. *)
+(*   Proof. rewrite /FromExist=><-. apply MUpd_exist. Qed. *)
+
+(*   Global Instance into_forall_MUpd {A} E1 E2 P (Φ : A → iProp) : *)
+(*     IntoForall P Φ → IntoForall (MUpd E1 E2 P) (λ a, MUpd E1 E2 (Φ a))%I. *)
+(*   Proof. rewrite /IntoForall=>->. apply MUpd_forall. Qed. *)
+
+(*   Global Instance from_modal_MUpd E P : *)
+(*     FromModal True modality_id (MUpd E E P) (MUpd E E P) P. *)
+(*   Proof. by rewrite /FromModal /= -MUpd_intro. Qed. *)
+
+(*   Global Instance from_modal_MUpd_wrong_mask E1 E2 P : *)
+(*     FromModal *)
+(*       (pm_error "Only non-mask-changing update modalities can be introduced directly. *)
+(* Use [iApply MUpd_mask_intro] to introduce mask-changing update modalities") *)
+(*       modality_id (MUpd E1 E2 P) (MUpd E1 E2 P) P | 100. *)
+(*   Proof. by intros []. Qed. *)
+
+(*   Global Instance elim_modal_bupd_MUpd *)
+(*          p E1 E2 P Q : *)
+(*     ElimModal True p false (|==> P) P (MUpd E1 E2 Q) (MUpd E1 E2 Q) | 10. *)
+(*   Proof. *)
+(*     unfold ElimModal. rewrite intuitionistically_if_elim. *)
+(*     rewrite (BUpd_MUpd E1). rewrite MUpd_frame_r. rewrite wand_elim_r. rewrite MUpd_trans. auto. *)
+(*   Qed. *)
+
+(*   Global Instance elim_modal_MUpd_MUpd_gen p E0 E1 E2 E3 P Q : *)
+(*     ElimModal (mset_sub E0 E2) p false (MUpd E0 E1 P) P (MUpd E2 E3 Q) (MUpd (E1 ++ mset_minus E2 E0) E3 Q). *)
+(*   Proof. *)
+(*     unfold ElimModal. i. rewrite intuitionistically_if_elim. *)
+(*     rewrite MUpd_frame_r. rewrite wand_elim_r. rewrite MUpd_mask_frame; eauto. *)
+(*   Qed. *)
+
+(*   Global Instance elim_modal_MUpd_MUpd p E1 E2 E3 P Q : *)
+(*     ElimModal True p false (MUpd E1 E2 P) P (MUpd E1 E3 Q) (MUpd E2 E3 Q). *)
+(*   Proof. *)
+(*     unfold ElimModal. rewrite intuitionistically_if_elim. *)
+(*     rewrite MUpd_frame_r. rewrite wand_elim_r. rewrite MUpd_trans. auto. *)
+(*   Qed. *)
+
+(*   Global Instance elim_modal_MUpd_MUpd_wrong_mask p E0 E1 E2 E3 P Q : *)
+(*     ElimModal *)
+(*       (pm_error "Goal and eliminated modality must have the same mask. *)
+(* Use [iMod (MUpd_mask_subseteq E2)] to adjust the mask of your goal to [E2]") *)
+(*       p false *)
+(*       (MUpd E1 E2 P) False (MUpd E0 E3 Q) False | 100. *)
+(*   Proof. intros []. Qed. *)
+
+(*   Global Instance add_modal_MUpd E1 E2 P Q : *)
+(*     AddModal (MUpd E1 E1 P) P (MUpd E1 E2 Q). *)
+(*   Proof. *)
+(*     unfold AddModal. rewrite MUpd_frame_r. rewrite wand_elim_r. rewrite MUpd_trans. auto. *)
+(*   Qed. *)
+
+(*   Global Instance elim_acc_MUpd {X} E1 E2 E α β mγ Q : *)
+(*     ElimAcc (X:=X) True (MUpd E1 E2) (MUpd E2 E1) α β mγ *)
+(*             (MUpd E1 E Q) *)
+(*             (λ x, MUpd E2 E2 (β x) ∗ (mγ x -∗? MUpd E1 E Q))%I. *)
+(*   Proof. *)
+(*     iIntros (_) "Hinner >Hacc". iDestruct "Hacc" as (x) "[Hα Hclose]". *)
+(*     iPoseProof ("Hinner" with "Hα") as "[> Hβ Hfin]". *)
+(*     iMod ("Hclose" with "Hβ") as "Hγ". by iApply "Hfin". *)
+(*   Qed. *)
+
+(*   Global Instance elim_modal_iupd_MUpd *)
+(*          p E1 E2 P Q : *)
+(*     ElimModal True p false (IUpd IA P) P (MUpd E1 E2 Q) (MUpd E1 E2 Q) | 10. *)
+(*   Proof. *)
+(*     unfold ElimModal. rewrite intuitionistically_if_elim. *)
+(*     i. iIntros "[H0 H1] [H2 H3]". *)
+(*     iPoseProof ("H0" with "H2") as "> [H2 H0]". *)
+(*     iApply ("H1" with "H0 [H2 H3]"). iFrame. *)
+(*   Qed. *)
+(* End MUPD. *)
+
+(* Ltac msubtac := *)
+(*   try by (ss; apply mset_sub_b_reflect; ss). *)
+
+(* #[export] Hint Unfold NatSort.sort: mset. *)
+(* Ltac msimpl := autounfold with mset; simpl. *)
 
 Lemma injective_map_NoDup_strong A B (f: A -> B) (l: list A)
       (INJ: forall a0 a1 (IN0: List.In a0 l) (IN1: List.In a1 l)
@@ -1502,24 +1459,24 @@ Proof.
   hexploit (INJ x a); eauto. i. subst. ss.
 Qed.
 
-Ltac iopen i H K :=
-  let str := constr:(String.append "[" (String.append H (String.append " " (String.append K "]")))) in
-  let Inv := fresh "I" in
-  evar (Inv: nat -> iProp);
-  ((iPoseProof (@MUpd_open _ Inv _ i) as "> _H";
-    [msubtac|
-      let x := (eval cbn in (Inv i)) in
-      change (Inv i) with x;
-      subst Inv;
-      msimpl;
-      iDestruct "_H" as str])
-   +
-     (iPoseProof (@MUpd_open _ Inv _ i) as "> _H";
-      [let x := (eval cbn in (Inv i)) in
-       change (Inv i) with x;
-       subst Inv;
-       msimpl;
-       iDestruct "_H" as str])).
+(* Ltac iopen i H K := *)
+(*   let str := constr:(String.append "[" (String.append H (String.append " " (String.append K "]")))) in *)
+(*   let Inv := fresh "I" in *)
+(*   evar (Inv: nat -> iProp); *)
+(*   ((iPoseProof (@MUpd_open _ Inv _ i) as "> _H"; *)
+(*     [msubtac| *)
+(*       let x := (eval cbn in (Inv i)) in *)
+(*       change (Inv i) with x; *)
+(*       subst Inv; *)
+(*       msimpl; *)
+(*       iDestruct "_H" as str]) *)
+(*    + *)
+(*      (iPoseProof (@MUpd_open _ Inv _ i) as "> _H"; *)
+(*       [let x := (eval cbn in (Inv i)) in *)
+(*        change (Inv i) with x; *)
+(*        subst Inv; *)
+(*        msimpl; *)
+(*        iDestruct "_H" as str])). *)
 
 
 Section UPDATING.
@@ -1546,6 +1503,32 @@ Section UPDATING.
   Qed.
 End UPDATING.
 
+Section LISTSUB.
+
+  Definition list_sub A (s0 s1: list A): Prop :=
+    exists s, Permutation (s ++ s0) s1.
+
+  Global Program Instance list_sub_PreOrder A: PreOrder (@list_sub A).
+  Next Obligation.
+  Proof.
+    ii. exists []. ss.
+  Qed.
+  Next Obligation.
+  Proof.
+    ii. unfold list_sub in *. des.
+    rewrite <- H in H0. exists (s ++ s0).
+    rewrite <- app_assoc. auto.
+  Qed.
+
+  Global Instance permutation_list_sub_proper A:
+    Proper (Permutation ==> Permutation ==> iff) (@list_sub A).
+  Proof.
+    ii. unfold list_sub. split.
+    { i. des. exists s. rewrite <- H. rewrite H1. auto. }
+    { i. des. exists s. rewrite H0. rewrite H. auto. }
+    Qed.
+
+End LISTSUB.
 
 
 Require Import Program.
@@ -2370,10 +2353,6 @@ Module Region.
     Qed.
   End REGION.
 End Region.
-
-Definition maps_to {Σ} {A: Type} {M: URA.t} `{ING: @GRA.inG (A ==> M)%ra Σ}
-           (a: A) (m: M): iProp :=
-  OwnM (maps_to_res a m).
 
 From Fairness Require Import NatStructsLarge.
 
