src/tlogic/TemporalLogic.v
@@ -1,28 +1,33 @@
 From stdpp Require Import coPset gmap namespaces.
 From sflib Require Import sflib.
-From Fairness Require PCM.
-From Fairness Require Import IProp IPM.
-From Fairness Require Import IndexedInvariants LogicSyntaxHOAS PCMForSyntax PCMEmbed.
+From Fairness Require Import PCM IProp IPM.
+From Fairness Require Import IndexedInvariants LogicSyntaxHOAS.
+(* From Fairness Require Import IndexedInvariants LogicSyntaxHOAS PCMForSyntax PCMEmbed. *)
 (* From Fairness Require Import ISim. *)
 From iris Require Import bi.big_op.
 From iris Require base_logic.lib.invariants.
 
 Local Notation index := nat.
 
-Module Atom.
+Section Atom.
+
+  Context `{Σ : GRA.t}.
+
+  Class Atom :=
+    { T : Type
+    ; interp : T -> iProp
+    }.
+
+End Atom.
+
+Module Atoms.
 
   Section ATOMS.
 
-    (* Context `{T : Type}. *)
+    Context `{Σ : GRA.t}.
 
-    Context `{σ : list PCMForSyntax.URA.t}.
-
-    (* TODO: more atoms *)
-
-    (* Atom do not interpret arguments. *)
     Inductive t {Typ : Syntax.type -> Type} : Type :=
-    | own {M : PCMForSyntax.URA.t} {IN : In M σ} (r : M)
-    (* | own {M : PCMForSyntax.URA.t} {IN : PCMForSyntax.GRA.inG M σ} (r : M) *)
+    | own {A : Atom} (a : A.(T))
     | owne (E : coPset)
     | ownd (D : gset positive)
     | owni (i : positive) (p : @Syntax.t Typ (@t Typ))
@@ -31,113 +36,67 @@ Module Atom.
     (* | own_inv_auth (ps : gmap positive (@Syntax.t Typ (@t Typ))) *)
     .
 
-    (* Inductive t {Typ : @Syntax.type T -> Type} : Type := *)
-    (* | owne (E : coPset) *)
-    (* | ownd (D : gset positive) *)
-    (* | owni (i : positive) (p : @Syntax.t T Typ (@t Typ)) *)
-    (* | syn_inv_auth_l (ps : list (prod positive (@Syntax.t T Typ (@t Typ)))) *)
-    (* (* Non strictly positive occurrence *) *)
-    (* (* | own_inv_auth (ps : gmap positive (@Syntax.t T Typ (@t Typ))) *) *)
-    (* . *)
-
   End ATOMS.
 
   Section INTERP.
 
-    Context `{σ : list PCMForSyntax.URA.t}.
-    (* Local Notation σ := (PCMForSyntax.GRA.of_list _σ). *)
-    (* Context `{σ : PCMForSyntax.GRA.t}. *)
     Context `{Σ : PCM.GRA.t}.
-    (* Context `{T : Type}. *)
-    (* Context `{TSem : T -> Type}. *)
-    Context `{SUB : forall M, In M σ -> PCM.GRA.inG (to_LURA M) Σ}.
 
-    (* This is too strong. *)
-    (* Context `{SUB : forall (M : URA.t), PCMForSyntax.GRA.inG M σ -> PCM.GRA.inG (to_LURA M) Σ}. *)
-
-    Local Notation typing := (@Syntax.Typ (@t σ)).
-    Local Notation Formulas := (fun (i : index) => @Syntax.t (typing i) (@t σ (typing i))).
-    (* Local Notation typing := (@Syntax.Typ T TSem (@t T)). *)
-    (* Local Notation Formulas := (fun (i : index) => @Syntax.t T (typing i) (@t T (typing i))). *)
+    Local Notation typing := (@Syntax.Typ (@t Σ)).
+    Local Notation Formulas := (fun (i : index) => @Syntax.t (typing i) (@t Σ (typing i))).
 
     Context `{@PCM.GRA.inG (IInvSetRA Formulas) Σ}.
     Context `{@PCM.GRA.inG (PCM.URA.pointwise index PCM.CoPset.t) Σ}.
     Context `{@PCM.GRA.inG (PCM.URA.pointwise index PCM.Gset.t) Σ}.
 
-    Definition to_semantics (n : index) (a : @t σ (typing n)) : iProp :=
+    Definition to_semantics (n : index) (a : @t Σ (typing n)) : iProp :=
       match a with
-      | @own _ _ M IN r => @OwnM Σ (to_LURA M) (SUB M IN) r
+      | @own _ _ A r => A.(interp) r
       | owne E => OwnE n E
       | ownd D => OwnD n D
       | owni i p => @OwnI Σ Formulas _ n i p
       | syn_inv_auth_l ps => @inv_auth Σ Formulas _ n (list_to_map ps)
       end.
 
-    (* Definition to_semantics (n : index) (a : @t T (typing n)) : iProp := *)
-    (*   match a with *)
-    (*   | owne E => OwnE n E *)
-    (*   | ownd D => OwnD n D *)
-    (*   | owni i p => @OwnI Σ Formulas _ n i p *)
-    (*   | syn_inv_auth_l ps => @inv_auth Σ Formulas _ n (list_to_map ps) *)
-    (*   end. *)
-
   End INTERP.
 
-End Atom.
+End Atoms.
 
 Section WSAT.
 
-  Context `{σ : list PCMForSyntax.URA.t}.
   Context `{Σ : PCM.GRA.t}.
-  Context `{SUB : forall M, In M σ -> PCM.GRA.inG (to_LURA M) Σ}.
-  (* Context `{Interp : Base.InterpMeta}. *)
 
-  (* Local Notation T := Base.t. *)
-  (* Local Notation TSem := (@Base.sem Base.interp). *)
-  (* Local Notation TSem := (Base.sem). *)
-
-  Local Notation typing := (@Syntax.Typ (@Atom.t σ)).
-  Local Notation Formulas := (fun (n : index) => @Syntax.t (typing n) (@Atom.t σ (typing n))).
-  (* Local Notation typing := (@Syntax.Typ T TSem (@Atom.t T)). *)
-  (* Local Notation Formulas := (fun (n : index) => @Syntax.t T (typing n) (@Atom.t T (typing n))). *)
+  Local Notation typing := (@Syntax.Typ (@Atoms.t Σ)).
+  Local Notation Formulas := (fun (n : index) => @Syntax.t (typing n) (@Atoms.t Σ (typing n))).
 
   Context `{@PCM.GRA.inG (IInvSetRA Formulas) Σ}.
   Context `{@PCM.GRA.inG (PCM.URA.pointwise index PCM.CoPset.t) Σ}.
   Context `{@PCM.GRA.inG (PCM.URA.pointwise index PCM.Gset.t) Σ}.
 
-  Local Notation AtomSem := (@Atom.to_semantics σ Σ SUB _).
-  Local Notation SynSem := (@Syntax.to_semantics Σ (@Atom.t σ) AtomSem).
-  (* Local Notation AtomSem := (@Atom.to_semantics Σ _ TSem _ _ _). *)
-  (* Local Notation SynSem := (@Syntax.to_semantics Σ _ TSem (@Atom.t T) AtomSem). *)
+  Local Notation AtomSem := (@Atoms.to_semantics Σ _ _ _).
+  Local Notation SynSem := (@Syntax.to_semantics Σ (@Atoms.t Σ) AtomSem).
 
-  Global Instance SynIISet : @IInvSet Σ Formulas := (@Syntax.IISet Σ (@Atom.t σ) AtomSem).
-  (* Global Instance SynIISet : @IInvSet Σ Formulas := (@Syntax.IISet Σ _ TSem (@Atom.t T) AtomSem). *)
+  Global Instance SynIISet : @IInvSet Σ Formulas := (@Syntax.IISet Σ (@Atoms.t Σ) AtomSem).
 
 
-  Definition syn_inv_auth n (ps : gmap positive (Formulas n)) : @Atom.t σ (typing n) :=
-    Atom.syn_inv_auth_l (map_to_list ps).
-  (* Definition syn_inv_auth n (ps : gmap positive (Formulas n)) : @Atom.t T (typing n) := *)
-  (*   Atom.syn_inv_auth_l (map_to_list ps). *)
+  Definition syn_inv_auth n (ps : gmap positive (Formulas n)) : @Atoms.t Σ (typing n) :=
+    Atoms.syn_inv_auth_l (map_to_list ps).
 
   Lemma syn_inv_auth_iProp
         n ps
     :
-    Atom.to_semantics n (syn_inv_auth n ps) = inv_auth n ps.
+    Atoms.to_semantics n (syn_inv_auth n ps) = inv_auth n ps.
   Proof.
     ss. rewrite list_to_map_to_list. ss.
   Qed.
 
-  Import Atom Syntax.
+  Import Atoms Syntax.
 
   Definition syn_inv_satall_fun n : positive -> (Formulas n) -> (Formulas n) :=
     fun i p => or (sepconj p (atom (ownd {[i]}))) (atom (owne {[i]})).
-  (* fun i p => Syntax.or (Syntax.sepconj p (Syntax.atom (ownd {[i]}))) (Syntax.atom (owne {[i]})). *)
 
   Definition syn_inv_satall n (ps : gmap positive (Formulas n)) : Formulas n :=
-    @star_gmap (@Atom.t σ) n ps (syn_inv_satall_fun n).
-    (* @star_gmap _ TSem (@Atom.t T) n ps (syn_inv_satall_fun n). *)
-  (* @Syntax.star_gmap _ TSem (@t T) n ps (inv_satall_fun n). *)
-
+    @star_gmap (@Atoms.t Σ) n ps (syn_inv_satall_fun n).
 
   Lemma syn_inv_satall_fun_iProp
         n i p
@@ -161,7 +120,6 @@ Section WSAT.
 
   Definition syn_wsat n : Formulas (S n) :=
     ex (pgmapT formulaT) (fun I => lift (sepconj (atom (syn_inv_auth n I)) (syn_inv_satall n I))).
-    (* ex (gmapTpos formulaT) (fun I => lift (sepconj (atom (syn_inv_auth n I)) (syn_inv_satall n I))). *)
 
   Lemma syn_wsat_iProp
         n
@@ -273,6 +231,73 @@ End FUPD.
     (* Set Printing All. *)
 
   End TEST.
+
+(* Module Atom. *)
+
+(*   Section ATOMS. *)
+
+(*     (* Context `{T : Type}. *) *)
+
+(*     Context `{σ : list PCMForSyntax.URA.t}. *)
+
+(*     (* TODO: more atoms *) *)
+
+(*     (* Atom do not interpret arguments. *) *)
+(*     Inductive t {Typ : Syntax.type -> Type} : Type := *)
+(*     | own {M : PCMForSyntax.URA.t} {IN : In M σ} (r : M) *)
+(*     (* | own {M : PCMForSyntax.URA.t} {IN : PCMForSyntax.GRA.inG M σ} (r : M) *) *)
+(*     | owne (E : coPset) *)
+(*     | ownd (D : gset positive) *)
+(*     | owni (i : positive) (p : @Syntax.t Typ (@t Typ)) *)
+(*     | syn_inv_auth_l (ps : list (prod positive (@Syntax.t Typ (@t Typ)))) *)
+(*     (* Non strictly positive occurrence *) *)
+(*     (* | own_inv_auth (ps : gmap positive (@Syntax.t Typ (@t Typ))) *) *)
+(*     . *)
+
+(*   End ATOMS. *)
+
+(*   Section INTERP. *)
+
+(*     Context `{σ : list PCMForSyntax.URA.t}. *)
+(*     (* Local Notation σ := (PCMForSyntax.GRA.of_list _σ). *) *)
+(*     (* Context `{σ : PCMForSyntax.GRA.t}. *) *)
+(*     Context `{Σ : PCM.GRA.t}. *)
+(*     (* Context `{T : Type}. *) *)
+(*     (* Context `{TSem : T -> Type}. *) *)
+(*     Context `{SUB : forall M, In M σ -> PCM.GRA.inG (to_LURA M) Σ}. *)
+
+(*     (* This is too strong. *) *)
+(*     (* Context `{SUB : forall (M : URA.t), PCMForSyntax.GRA.inG M σ -> PCM.GRA.inG (to_LURA M) Σ}. *) *)
+
+(*     Local Notation typing := (@Syntax.Typ (@t σ)). *)
+(*     Local Notation Formulas := (fun (i : index) => @Syntax.t (typing i) (@t σ (typing i))). *)
+(*     (* Local Notation typing := (@Syntax.Typ T TSem (@t T)). *) *)
+(*     (* Local Notation Formulas := (fun (i : index) => @Syntax.t T (typing i) (@t T (typing i))). *) *)
+
+(*     Context `{@PCM.GRA.inG (IInvSetRA Formulas) Σ}. *)
+(*     Context `{@PCM.GRA.inG (PCM.URA.pointwise index PCM.CoPset.t) Σ}. *)
+(*     Context `{@PCM.GRA.inG (PCM.URA.pointwise index PCM.Gset.t) Σ}. *)
+
+(*     Definition to_semantics (n : index) (a : @t σ (typing n)) : iProp := *)
+(*       match a with *)
+(*       | @own _ _ M IN r => @OwnM Σ (to_LURA M) (SUB M IN) r *)
+(*       | owne E => OwnE n E *)
+(*       | ownd D => OwnD n D *)
+(*       | owni i p => @OwnI Σ Formulas _ n i p *)
+(*       | syn_inv_auth_l ps => @inv_auth Σ Formulas _ n (list_to_map ps) *)
+(*       end. *)
+
+(*     (* Definition to_semantics (n : index) (a : @t T (typing n)) : iProp := *) *)
+(*     (*   match a with *) *)
+(*     (*   | owne E => OwnE n E *) *)
+(*     (*   | ownd D => OwnD n D *) *)
+(*     (*   | owni i p => @OwnI Σ Formulas _ n i p *) *)
+(*     (*   | syn_inv_auth_l ps => @inv_auth Σ Formulas _ n (list_to_map ps) *) *)
+(*     (*   end. *) *)
+
+(*   End INTERP. *)
+
+(* End Atom. *)
 
 
   (* Definition inv (N : namespace) P := *)
