src/tlogic/IPropAux.v
@@ -1,0 +1,231 @@
+From sflib Require Import sflib.
+Require Import Program.
+From Fairness Require Import PCM IProp IPM.
+From Fairness Require Import Axioms.
+
+Set Implicit Arguments.
+
+Section AUX.
+
+  Lemma embed_core_commute `{@GRA.inG M Σ}
+        (r: M)
+    :
+    GRA.embed (URA.core r) = URA.core (GRA.embed r).
+  Proof.
+    Local Transparent GRA.to_URA URA.unit.
+    dependent destruction H. subst.
+    extensionality n. ss. unfold URA.core at 2. ss.
+    unfold GRA.embed. destruct (PeanoNat.Nat.eq_dec GRA.inG_id n) eqn:EQ; ss.
+    { subst. ss. }
+    { des_ifs. ss. transitivity (add (core unit) unit); auto. }
+  Qed.
+
+  Lemma own_persistent `{@GRA.inG M Σ}
+        (r: M)
+    :
+    (OwnM r) -∗ (□ OwnM (URA.core r)).
+  Proof.
+    rr. autorewrite with iprop. i.
+    rr. autorewrite with iprop. split.
+    { rr. autorewrite with iprop. auto. }
+    { rr. autorewrite with iprop.
+      rr in H0. autorewrite with iprop in H0.
+      rr. autorewrite with iprop.
+      eapply URA.extends_core in H0.
+      rewrite embed_core_commute. auto.
+    }
+  Qed.
+
+  Lemma OwnM_ura_unit `{@GRA.inG M Σ}
+    :
+    ⊢ OwnM (@URA.unit M).
+  Proof.
+    rr. autorewrite with iprop. i.
+    rr. autorewrite with iprop.
+    exists r.
+    Local Transparent GRA.to_URA URA.unit.
+    replace (GRA.embed ε) with (@URA.unit Σ).
+    { rewrite URA.unit_idl. auto. }
+    unfold GRA.embed. extensionality n. des_ifs. ss.
+    destruct H. ss. destruct inG_prf. ss.
+  Qed.
+
+End AUX.
+
+Definition maps_to {Σ} {A: Type} {M: URA.t} `{ING: @GRA.inG (A ==> M)%ra Σ}
+           (a: A) (m: M): iProp :=
+  OwnM (maps_to_res a m).
+
+Section UPD.
+  Variable A: Type.
+  Context `{IN: @GRA.inG (Auth.t (Excl.t A)) Σ}.
+
+  Lemma black_white_update a0 a' a1
+    :
+    (OwnM (Auth.black (Excl.just a0: @Excl.t A)))
+      -∗
+      (OwnM (Auth.white (Excl.just a': @Excl.t A)))
+      -∗
+      #=> (OwnM (Auth.black (Excl.just a1: @Excl.t A)) ** OwnM (Auth.white (Excl.just a1: @Excl.t A))).
+  Proof.
+    iIntros "H0 H1". iCombine "H0 H1" as "H".
+    iPoseProof (OwnM_Upd with "H") as "> [H0 H1]".
+    { apply Auth.auth_update.
+      instantiate (1:=Excl.just a1). instantiate (1:=Excl.just a1).
+      ii. des. ur in FRAME. des_ifs. split.
+      { ur. ss. }
+      { ur. ss. }
+    }
+    iModIntro. iFrame.
+  Qed.
+
+  Lemma black_white_equal a a'
+    :
+    (OwnM (Auth.black (Excl.just a: @Excl.t A)))
+      -∗
+      (OwnM (Auth.white (Excl.just a': @Excl.t A)))
+      -∗
+      ⌜a = a'⌝.
+  Proof.
+    iIntros "H0 H1". iCombine "H0 H1" as "H".
+    iOwnWf "H". ur in H. des.
+    rr in H. des. ur in H. des_ifs.
+  Qed.
+
+  Lemma white_white_excl a a'
+    :
+    (OwnM (Auth.white (Excl.just a: @Excl.t A)))
+      -∗
+      (OwnM (Auth.white (Excl.just a': @Excl.t A)))
+      -∗
+      ⌜False⌝.
+  Proof.
+    iIntros "H0 H1". iCombine "H0 H1" as "H".
+    iOwnWf "H". ur in H. ur in H. auto.
+  Qed.
+
+End UPD.
+
+Section OWNS.
+
+  Variable (Id: Type).
+  Context `{R: URA.t}.
+  Context `{IN1: @GRA.inG R Σ}.
+  Context `{IN2: @GRA.inG (Id ==> R)%ra Σ}.
+
+  Definition OwnMs (s: Id -> Prop) (u: R): iProp :=
+    (OwnM ((fun i =>
+              if (excluded_middle_informative (s i))
+              then u
+              else ε): (Id ==> R)%ra)).
+
+  Lemma OwnMs_impl (s0 s1: Id -> Prop) u
+        (IMPL: forall i (IN: s0 i), s1 i)
+    :
+    (OwnMs s1 u)
+      -∗
+      (OwnMs s0 u).
+  Proof.
+    iIntros "OWNMS".
+    iApply (OwnM_extends with "OWNMS"). apply pointwise_extends.
+    i. des_ifs; try by reflexivity.
+    { exfalso. eauto. }
+    { eexists _. rewrite URA.unit_idl. ss. }
+  Qed.
+
+  Lemma OwnMs_empty s u
+        (EMPTY: forall i, ~ s i)
+    :
+    ⊢ OwnMs s u.
+  Proof.
+    iIntros. iApply (OwnM_extends with "[]").
+    2:{ iApply (@OwnM_ura_unit (Id ==> R)%ra). }
+    apply pointwise_extends. i. des_ifs.
+    { exfalso. eapply EMPTY; eauto. }
+    eexists _. rewrite URA.unit_idl. eauto.
+  Qed.
+
+  Lemma OwnMs_fold (s0 s1: Id -> Prop) i u
+        (IMPL: forall j (IN: s0 j), s1 j \/ j = i)
+    :
+    ((OwnMs s1 u) ** (maps_to i u))
+      -∗
+      (OwnMs s0 u).
+  Proof.
+    iIntros "[OWNMS OWN]".
+    iCombine "OWNMS OWN" as "OWNMS".
+    iApply (OwnM_extends with "OWNMS"). apply pointwise_extends.
+    i. erewrite ! (@unfold_pointwise_add Id R). unfold maps_to_res.
+    des_ifs; ss; repeat rewrite URA.unit_id; repeat rewrite URA.unit_idl; ss; try by reflexivity.
+    { eexists. apply URA.add_comm. }
+    { hexploit IMPL; eauto. i. des; ss. }
+    { eexists. rewrite URA.unit_idl. ss. }
+    { eexists. rewrite URA.unit_idl. ss. }
+    { eexists. rewrite URA.unit_idl. ss. }
+  Qed.
+
+  Definition OwnMs_unfold (s0 s1: Id -> Prop) i u
+             (IMPL: forall j (IN: s0 j \/ j = i), s1 j)
+             (NIN: ~ s0 i)
+    :
+    (OwnMs s1 u)
+      -∗
+      (OwnMs s0 u ** maps_to i u).
+  Proof.
+    iIntros "OWNMS".
+    iPoseProof (OwnM_extends with "OWNMS") as "[OWNMS0 OWNMS1]".
+    { instantiate (1:=maps_to_res i (u: R): (Id ==> R)%ra).
+      instantiate (1:=(fun i =>
+                         if (excluded_middle_informative (s0 i))
+                         then u
+                         else ε)).
+      erewrite ! (@unfold_pointwise_add Id R). unfold maps_to_res.
+      apply pointwise_extends. i.
+      des_ifs; ss; repeat rewrite URA.unit_id; repeat rewrite URA.unit_idl; ss; try by reflexivity.
+      { exfalso. eapply n0. auto. }
+      { exfalso. eapply n0. auto. }
+      { eexists. rewrite URA.unit_idl. ss. }
+    }
+    iFrame.
+  Qed.
+
+  Definition OwnMs_combine (s0 s1: Id -> Prop) u
+    :
+    (OwnMs s0 u ** OwnMs s1 u)
+      -∗
+      (OwnMs (fun i => s0 i \/ s1 i) u).
+  Proof.
+    iIntros "[OWNMS0 OWNMS1]".
+    iCombine "OWNMS0 OWNMS1" as "OWNMS".
+    iApply (OwnM_extends with "OWNMS"). apply pointwise_extends.
+    i. erewrite ! (@unfold_pointwise_add Id R).
+    des_ifs; ss; repeat rewrite URA.unit_id; repeat rewrite URA.unit_idl; ss; try by reflexivity.
+    { eexists. eauto. }
+    { des; ss. }
+    { eexists. rewrite URA.unit_idl. ss. }
+    { eexists. rewrite URA.unit_idl. ss. }
+    { eexists. rewrite URA.unit_idl. ss. }
+  Qed.
+
+  Definition OwnMs_split (s0 s1: Id -> Prop) u
+             (DISJOINT: forall i (IN0: s0 i) (IN1: s1 i), False)
+    :
+    (OwnMs (fun i => s0 i \/ s1 i) u)
+      -∗
+      (OwnMs s0 u ** OwnMs s1 u).
+  Proof.
+    iIntros "OWNMS".
+    iPoseProof (OwnM_extends with "OWNMS") as "[OWNMS0 OWNMS1]".
+    2:{ iSplitL "OWNMS0"; [iExact "OWNMS0"|iExact "OWNMS1"]. }
+    { apply pointwise_extends.
+      i. erewrite ! (@unfold_pointwise_add Id R).
+      des_ifs; ss; repeat rewrite URA.unit_id; repeat rewrite URA.unit_idl; ss; try by reflexivity.
+      { exfalso. eapply DISJOINT; eauto. }
+      { exfalso. eapply n; eauto. }
+      { exfalso. eapply n0; eauto. }
+      { exfalso. eapply n0; eauto. }
+      { des; ss. }
+    }
+  Qed.
+
+End OWNS.
